BIL_Syntax.thy
@@ -139,21 +139,59 @@ where
   \<open>wfe (Concat e\<^sub>1 e\<^sub>2) = (wfe e\<^sub>1 \<and> wfe e\<^sub>2)\<close> |
   \<open>wfe _ = True\<close>
 
-(*TODO capture-avoiding? *)
+class capture_avoiding_sub =
+  fixes let_substitute :: \<open>'a \<Rightarrow> var \<Rightarrow> exp \<Rightarrow> exp\<close> (\<open>[_\<sslash>_]_\<close>)
+
+instantiation exp :: capture_avoiding_sub
+begin
+
 primrec 
-  let_substitute_val :: \<open>exp \<Rightarrow> var \<Rightarrow> exp \<Rightarrow> exp\<close> (\<open>[_\<sslash>_]_\<close>)
+  let_substitute_exp :: \<open>exp \<Rightarrow> var \<Rightarrow> exp \<Rightarrow> exp\<close>
 where
-  \<open>([_\<sslash>_](Val v)) = (Val v)\<close> |
-  \<open>([e\<sslash>var](Var var')) = (if var = var' then e else (Var var'))\<close> |
-  \<open>([e\<sslash>var](Load e\<^sub>1 e\<^sub>2 ed sz)) = Load ([e\<sslash>var]e\<^sub>1) ([e\<sslash>var]e\<^sub>2) ed sz\<close> |
-  \<open>([e\<sslash>var](Store e\<^sub>1 e\<^sub>2 ed sz e\<^sub>3)) = Store ([e\<sslash>var]e\<^sub>1) ([e\<sslash>var]e\<^sub>2) ed sz ([e\<sslash>var]e\<^sub>3)\<close> |
-  \<open>([e\<sslash>var](BinOp e\<^sub>1 bop e\<^sub>2)) = BinOp ([e\<sslash>var]e\<^sub>1) bop ([e\<sslash>var]e\<^sub>2)\<close> |
-  \<open>([e\<sslash>var](UnOp uop e')) = UnOp uop ([e\<sslash>var]e')\<close> |
-  \<open>([e\<sslash>var](Cast cast sz e')) = Cast cast sz ([e\<sslash>var]e')\<close> |
-  \<open>([e\<sslash>var](Let var' e\<^sub>1 e\<^sub>2)) = Let var' ([e\<sslash>var]e\<^sub>1) ([e\<sslash>var]e\<^sub>2)\<close> |
-  \<open>([e\<sslash>var](Ite e\<^sub>1 e\<^sub>2 e\<^sub>3)) = Ite ([e\<sslash>var]e\<^sub>1) ([e\<sslash>var]e\<^sub>2) ([e\<sslash>var]e\<^sub>3)\<close> |
-  \<open>([e\<sslash>var](Extract sz\<^sub>1 sz\<^sub>2 e')) = Extract sz\<^sub>1 sz\<^sub>2 ([e\<sslash>var]e')\<close> |
-  \<open>([e\<sslash>var](Concat e\<^sub>1 e\<^sub>2)) = Concat ([e\<sslash>var]e\<^sub>1) ([e\<sslash>var]e\<^sub>2)\<close>
+  \<open>let_substitute_exp _ _ (Val v) = (Val v)\<close> |
+  \<open>let_substitute_exp e var (Var var') = (if var = var' then e else (Var var'))\<close> |
+  \<open>let_substitute_exp e var (Load e\<^sub>1 e\<^sub>2 ed sz) = Load (let_substitute_exp e var e\<^sub>1) (let_substitute_exp e var e\<^sub>2) ed sz\<close> |
+  \<open>let_substitute_exp e var (Store e\<^sub>1 e\<^sub>2 ed sz e\<^sub>3) = Store (let_substitute_exp e var e\<^sub>1) (let_substitute_exp e var e\<^sub>2) ed sz (let_substitute_exp e var e\<^sub>3)\<close> |
+  \<open>let_substitute_exp e var (BinOp e\<^sub>1 bop e\<^sub>2) = BinOp (let_substitute_exp e var e\<^sub>1) bop (let_substitute_exp e var e\<^sub>2)\<close> |
+  \<open>let_substitute_exp e var (UnOp uop e') = UnOp uop (let_substitute_exp e var e')\<close> |
+  \<open>let_substitute_exp e var (Cast cast sz e') = Cast cast sz (let_substitute_exp e var e')\<close> |
+  \<open>let_substitute_exp e var (Let var' e\<^sub>1 e\<^sub>2) = Let var' (let_substitute_exp e var e\<^sub>1) (let_substitute_exp e var e\<^sub>2)\<close> |
+  \<open>let_substitute_exp e var (Ite e\<^sub>1 e\<^sub>2 e\<^sub>3) = Ite (let_substitute_exp e var e\<^sub>1) (let_substitute_exp e var e\<^sub>2) (let_substitute_exp e var e\<^sub>3)\<close> |
+  \<open>let_substitute_exp e var (Extract sz\<^sub>1 sz\<^sub>2 e') = Extract sz\<^sub>1 sz\<^sub>2 (let_substitute_exp e var e')\<close> |
+  \<open>let_substitute_exp e var (Concat e\<^sub>1 e\<^sub>2) = Concat (let_substitute_exp e var e\<^sub>1) (let_substitute_exp e var e\<^sub>2)\<close>
+
+instance ..
+end 
+
+instantiation val :: capture_avoiding_sub
+begin
+
+primrec 
+  let_substitute_val :: \<open>val \<Rightarrow> var \<Rightarrow> exp \<Rightarrow> exp\<close>
+where
+  \<open>let_substitute_val _ _ (Val v) = (Val v)\<close> |
+  \<open>let_substitute_val v var (Var var') = (if var = var' then (Val v) else (Var var'))\<close> |
+  \<open>let_substitute_val v var (Load e\<^sub>1 e\<^sub>2 ed sz) = Load (let_substitute_val v var e\<^sub>1) (let_substitute_val v var e\<^sub>2) ed sz\<close> |
+  \<open>let_substitute_val v var (Store e\<^sub>1 e\<^sub>2 ed sz e\<^sub>3) = Store (let_substitute_val v var e\<^sub>1) (let_substitute_val v var e\<^sub>2) ed sz (let_substitute_val v var e\<^sub>3)\<close> |
+  \<open>let_substitute_val v var (BinOp e\<^sub>1 bop e\<^sub>2) = BinOp (let_substitute_val v var e\<^sub>1) bop (let_substitute_val v var e\<^sub>2)\<close> |
+  \<open>let_substitute_val v var (UnOp uop e') = UnOp uop (let_substitute_val v var e')\<close> |
+  \<open>let_substitute_val v var (Cast cast sz e') = Cast cast sz (let_substitute_val v var e')\<close> |
+  \<open>let_substitute_val v var (Let var' e\<^sub>1 e\<^sub>2) = Let var' (let_substitute_val v var e\<^sub>1) (let_substitute_val v var e\<^sub>2)\<close> |
+  \<open>let_substitute_val v var (Ite e\<^sub>1 e\<^sub>2 e\<^sub>3) = Ite (let_substitute_val v var e\<^sub>1) (let_substitute_val v var e\<^sub>2) (let_substitute_val v var e\<^sub>3)\<close> |
+  \<open>let_substitute_val v var (Extract sz\<^sub>1 sz\<^sub>2 e') = Extract sz\<^sub>1 sz\<^sub>2 (let_substitute_val v var e')\<close> |
+  \<open>let_substitute_val v var (Concat e\<^sub>1 e\<^sub>2) = Concat (let_substitute_val v var e\<^sub>1) (let_substitute_val v var e\<^sub>2)\<close>
+
+instance ..
+end 
+
+lemma let_substitue_val_exp_val_eq:
+  \<open>[v\<sslash>var]e = [(Val v)\<sslash>var]e\<close>
+  by (induct e, auto)
+  
+lemma let_substitute_val_size_eq: 
+    fixes v :: val
+    shows \<open>size_class.size e = size_class.size ([v\<sslash>var]e)\<close>
+  by (induct e, auto)
 
 datatype stmt =
     Move var exp
