BIR_Syntax.thy
@@ -385,25 +385,416 @@ where
   \<open>wf\<Delta> \<Delta> \<equiv> (\<forall>var \<in> dom \<Delta>. snd var = type (the (\<Delta> var))) \<and>
             (\<forall>var \<in> dom \<Delta>. var \<noteq> mem \<longrightarrow> (\<exists>sz. snd var = Imm sz))\<close>
 
+lemma \<Gamma>_val_imm_not_storage:
+  assumes \<open>\<Gamma> \<turnstile> v :: Imm sz\<close>
+    shows \<open>v \<noteq> Storage x31 x32 x33 x34\<close>
+  using assms by (induct v, auto)
+
+lemma \<Gamma>_val_mem_not_immediate:
+  assumes \<open>\<Gamma> \<turnstile> v :: Mem sz1 sz2\<close>
+    shows \<open>v \<noteq> Immediate w\<close>
+  using assms by (induct v, auto)
+
 lemma \<Gamma>_val_type_implies_type_t:
   assumes \<open>\<Gamma> \<turnstile> v :: t\<close>
     shows \<open>type v = t\<close>
-  using assms apply (induct v)
+  using assms by (induct rule: typing_expression_val_induct, auto)
+
+lemma \<Gamma>_val_implies_load_val:
+  assumes \<open>\<Gamma> \<turnstile> v :: (Mem sz\<^sub>a\<^sub>d\<^sub>d\<^sub>r sz\<^sub>m\<^sub>e\<^sub>m)\<close>
+    shows \<open>\<Gamma> \<turnstile> load_val v w\<^sub>a\<^sub>d\<^sub>d\<^sub>r :: (Imm sz\<^sub>m\<^sub>e\<^sub>m)\<close>
+  using assms apply (induct v, auto)
+  apply (metis Bitvector_Syntax.word.exhaust typing_expression_val.simps(3))
+  by (metis Bitvector_Syntax.word.exhaust typing_expression_val.simps(3))
+
+lemma \<Gamma>_val_implies_load_val_en:
+  assumes \<open>\<Gamma> \<turnstile> v :: (Mem sz\<^sub>a\<^sub>d\<^sub>d\<^sub>r sz\<^sub>m\<^sub>e\<^sub>m)\<close>
+    shows \<open>\<Gamma> \<turnstile> load_val_en v sz\<^sub>m\<^sub>e\<^sub>m w sz\<^sub>v\<^sub>a\<^sub>l ed :: (Imm sz\<^sub>v\<^sub>a\<^sub>l)\<close>
+  using assms
+  apply (induct ed, auto)
+  apply (induct "(sz\<^sub>v\<^sub>a\<^sub>l div sz\<^sub>m\<^sub>e\<^sub>m - Suc 0)")
   apply auto
-  using typing_expression_val.elims(2) apply fastforce
-  apply (subgoal_tac \<open>\<exists>sz\<^sub>a\<^sub>d\<^sub>d\<^sub>r sz\<^sub>v\<^sub>a\<^sub>l. t = (Mem sz\<^sub>a\<^sub>d\<^sub>d\<^sub>r sz\<^sub>v\<^sub>a\<^sub>l)\<close>)
-  apply force
-  by (metis Type.exhaust typing_expression_val.simps(4))
+  defer
+  oops
+
+(*
+thm load_val_be.induct
+lemma load_val_be_induct[consumes 1, case_names ReadSingleByte ReadManyBytes]:
+  assumes \<open>v' = load_val_be v w n\<close>
+      and \<open>\<lbrakk>v' = load_val v w\<rbrakk> \<Longrightarrow> P v w 0\<close>
+      and \<open>(\<And>n w v v' w\<^sub>c\<^sub>o\<^sub>n\<^sub>c\<^sub>a\<^sub>t. \<lbrakk>Immediate w\<^sub>c\<^sub>o\<^sub>n\<^sub>c\<^sub>a\<^sub>t = load_val_be v (succ w) n; v' = load_val v w\<rbrakk> \<Longrightarrow> P v w (Suc n))\<close>
+    shows \<open>P v w n\<close>
+  using assms apply (induct rule: load_val_be.induct)
+  apply auto[1]
+  apply (simp only: load_val_be.simps)
+
+thm load_val_en.induct
+lemma load_val_en_induct[consumes 1, case_names ReadSingleByte ReadByteBigEndian ReadByteLittleEndian]:
+  assumes \<open>v' = load_val_en v sz\<^sub>m\<^sub>e\<^sub>m w sz\<^sub>v\<^sub>a\<^sub>l en\<close>
+      and \<open>(\<And>a. \<lbrakk>sz\<^sub>v\<^sub>a\<^sub>l div sz\<^sub>m\<^sub>e\<^sub>m = 1; v' = load_val v w\<rbrakk> \<Longrightarrow> P v sz\<^sub>m\<^sub>e\<^sub>m w sz\<^sub>v\<^sub>a\<^sub>l en)\<close>
+      and \<open>(\<And>a. \<lbrakk>sz\<^sub>v\<^sub>a\<^sub>l div sz\<^sub>m\<^sub>e\<^sub>m > 1; v' = load_val v w\<rbrakk> \<Longrightarrow> P v sz\<^sub>m\<^sub>e\<^sub>m w sz\<^sub>v\<^sub>a\<^sub>l be)\<close>
+      and \<open>(\<And>a. \<lbrakk>sz\<^sub>v\<^sub>a\<^sub>l div sz\<^sub>m\<^sub>e\<^sub>m > 1; v' = load_val v w\<rbrakk> \<Longrightarrow> P v sz\<^sub>m\<^sub>e\<^sub>m w sz\<^sub>v\<^sub>a\<^sub>l el)\<close>
+    shows \<open>P v sz\<^sub>m\<^sub>e\<^sub>m w sz\<^sub>v\<^sub>a\<^sub>l en\<close>
+  using assms apply (cases en, auto)
+  apply (cases \<open>sz\<^sub>v\<^sub>a\<^sub>l div sz\<^sub>m\<^sub>e\<^sub>m = Suc 0\<close>, auto)
+  sledgehammer
+*)
+thm eval_exp.induct
+lemma typing_expression_exp_implies_eval_exp:
+  assumes \<open>\<Gamma> \<turnstile> e :: t\<close>
+    shows \<open>\<Gamma> \<turnstile> (eval_exp \<Delta> e) :: t\<close>
+using assms proof (induct rule: typing_expression_exp_induct)
+  case (Val \<Gamma> v t)
+  then show ?case by auto
+next
+  case (Var \<Gamma> name t)
+  then show ?case apply auto sorry
+next
+  case (Load \<Gamma> e\<^sub>1 e\<^sub>2 ed sz sz\<^sub>a\<^sub>d\<^sub>d\<^sub>r sz\<^sub>m\<^sub>e\<^sub>m t)
+  have el_valid: "\<And>v w. \<Gamma> \<turnstile> load_val_el v w (sz div sz\<^sub>m\<^sub>e\<^sub>m - Suc 0) :: Imm sz"
+    sorry
+  have be_valid: "\<And>v w v' w'. \<Gamma> \<turnstile> load_val_be v w' (sz div sz\<^sub>m\<^sub>e\<^sub>m - Suc 0) :: Imm sz"
+    sorry
+  show ?case
+    using Load apply (auto simp add: Let_def)
+    apply (cases \<open>eval_exp \<Delta> e\<^sub>1\<close>, auto)
+    apply (cases \<open>eval_exp \<Delta> e\<^sub>2\<close>, auto)
+    apply (drule_tac typing_val_storage)
+    apply (drule_tac typing_val_immediate)
+    using el_valid be_valid by (cases ed, auto)
+next
+  case (Store \<Gamma> sz\<^sub>a\<^sub>d\<^sub>d\<^sub>r sz\<^sub>m\<^sub>e\<^sub>m sz\<^sub>v\<^sub>a\<^sub>l e\<^sub>1 e\<^sub>2 ed e\<^sub>3 t)
+  then show ?case 
+    apply (auto simp add: Let_def)
+    apply (cases \<open>eval_exp \<Delta> e\<^sub>2\<close>)
+    using \<Gamma>_val_type_implies_type_t apply auto
+    sorry
+next
+  case (BinAOp \<Gamma> e\<^sub>1 aop e\<^sub>2 sz t)
+  then show ?case 
+    apply (cases \<open>eval_exp \<Delta> e\<^sub>1\<close>, auto)
+    apply (cases \<open>eval_exp \<Delta> e\<^sub>2\<close>, auto)
+    using typing_val_immediate by (case_tac aop, auto)
+next
+  case (BinLOp \<Gamma> e\<^sub>1 lop e\<^sub>2 sz t)
+  then show ?case 
+    apply (cases \<open>eval_exp \<Delta> e\<^sub>1\<close>, auto)
+    apply (cases \<open>eval_exp \<Delta> e\<^sub>2\<close>, auto)
+    using typing_val_immediate by (case_tac lop, auto)
+next
+  case (UOp \<Gamma> uop e sz t)
+  then show ?case 
+    apply (cases \<open>eval_exp \<Delta> e\<close>, auto)
+    using typing_val_immediate by (case_tac uop, auto)
+next
+  case (UnsignedCast \<Gamma> e sz sz' t)
+  then show ?case 
+    using typing_val_implies_valid_context by (cases \<open>eval_exp \<Delta> e\<close>, auto)
+next
+  case (SignedCast \<Gamma> e sz sz' t)
+  then show ?case 
+    using typing_val_implies_valid_context by (cases \<open>eval_exp \<Delta> e\<close>, auto)
+next
+  case (HighCast \<Gamma> e sz sz' t)
+  then show ?case 
+    using typing_val_implies_valid_context apply (cases \<open>eval_exp \<Delta> e\<close>, auto)
+    using Suc_diff_Suc diff_diff_cancel diff_less typing_val_immediate by presburger
+next
+  case (LowCast \<Gamma> e sz sz' t)
+  then show ?case 
+    using typing_val_implies_valid_context by (cases \<open>eval_exp \<Delta> e\<close>, auto)
+next
+  case (Let \<Gamma> name t' e\<^sub>1 e\<^sub>2 t)
+  then show ?case
+    apply (subgoal_tac \<open>\<Gamma> \<turnstile> eval_exp \<Delta> e\<^sub>2 :: t\<close>) defer
+    using typing_expression_\<Gamma>_extend_implies_\<Gamma> apply blast
+    apply auto
+    apply (induct \<Delta> "[eval_exp \<Delta> e\<^sub>1\<sslash>(name, t')]e\<^sub>2" rule: eval_exp.induct)
+    apply auto
+    sledgehammer
+
+    apply (cases \<open>eval_exp \<Delta> e\<^sub>1\<close>, auto)
+
+    sorry
+next
+  case (Ite \<Gamma> e\<^sub>1 e\<^sub>2 e\<^sub>3 t)
+  then show ?case 
+    apply (auto simp add: Let_def)
+    apply (cases \<open>eval_exp \<Delta> e\<^sub>1\<close>, auto)
+    by (simp_all add: \<Gamma>_val_type_implies_type_t typing_val_implies_valid_t)
+next
+  case (Extract \<Gamma> sz\<^sub>1 sz\<^sub>2 sz\<^sub>e\<^sub>x\<^sub>t\<^sub>r\<^sub>a\<^sub>c\<^sub>t sz e t)
+  then show ?case 
+    using typing_val_implies_valid_context by (cases \<open>eval_exp \<Delta> e\<close>, auto)
+next
+  case (Concat \<Gamma> e\<^sub>1 e\<^sub>2 sz\<^sub>c\<^sub>o\<^sub>n\<^sub>c\<^sub>a\<^sub>t sz\<^sub>1 sz\<^sub>2 t)
+  then show ?case 
+    apply (cases \<open>eval_exp \<Delta> e\<^sub>1\<close>, auto)
+    using typing_val_immediate apply (cases \<open>eval_exp \<Delta> e\<^sub>2\<close>, auto)
+    by (simp add: \<Gamma>_val_type_implies_type_t)
+qed
+(*
+lemma \<Gamma>_exp_mem_not_immediate:
+  assumes \<open>\<Gamma> \<turnstile> e :: t\<close>
+      and \<open>t = Mem sz1 sz2\<close>
+    shows \<open>eval_exp \<Delta> e \<noteq> Immediate w\<close>
+  using assms apply (induct rule: typing_expression_exp.induct)
+  apply (auto simp add: Let_def)
+  defer (* invariant *)
+
+  apply (case_tac \<open>type (eval_exp \<Delta> e\<^sub>1)\<close>, auto)
+  defer (* enforce type (eval_exp \<Delta> e\<^sub>1) must be mem *)
+  apply (case_tac \<open>eval_exp \<Delta> e\<^sub>2\<close>, auto)
+  sledgehammer
+
+
+  using assms apply (induct rule: eval_exp.induct)
+  apply auto
+     
+     
+     defer
+
+  
+
+  case (Val x)
+  then show ?case by auto
+next
+  case (Var x)
+  then show ?case by auto
+next
+  case (Load e1 e2 x3 x4)
+  then show ?case by auto
+next
+  case (Store e1 e2 x3 x4 e3)
+  then show ?case sorry
+next
+  case (BinOp e1 x2a e2)
+  then show ?case by auto
+next
+  case (UnOp x1a e)
+  then show ?case by auto
+next
+  case (Cast x1a x2a e)
+  then show ?case by auto
+next
+  case (Let x1a e1 e2)
+  then show ?case     
+    apply (induct \<open>x1a\<close>, auto)
+    sorry
+next
+  case (Ite e1 e2 e3)
+  then show ?case 
+    apply (auto simp add: Let_def)
+    apply (cases \<open>eval_exp \<Delta> e1\<close>)
+    apply auto
+    apply (smt (verit, ccfv_SIG) val.simps(10))
+    sorry
+
+next
+  case (Extract x1a x2a e)
+  then show ?case by auto
+next
+  case (Concat e1 e2)
+  then show ?case by auto
+qed
+  
+*)
+(*
+lemma ZZ:
+  assumes \<open>\<Gamma> \<turnstile> e :: t\<close>
+      and \<open>t = Imm sz\<close>
+    shows \<open>eval_exp \<Delta> e \<noteq> Storage x31 x32 x33 x34\<close>
+using assms proof (induct rule: typing_expression_exp_induct)
+  case (Val \<Gamma> v t)
+  then show ?case by auto
+next
+  case (Var \<Gamma> name t)
+  then show ?case sorry
+next
+  case (Load \<Gamma> e\<^sub>1 e\<^sub>2 ed sz sz\<^sub>a\<^sub>d\<^sub>d\<^sub>r sz\<^sub>m\<^sub>e\<^sub>m t)
+  then show ?case 
+    apply (auto simp add: Let_def) sorry
+next
+  case (Store \<Gamma> sz\<^sub>a\<^sub>d\<^sub>d\<^sub>r sz\<^sub>m\<^sub>e\<^sub>m sz\<^sub>v\<^sub>a\<^sub>l e\<^sub>1 e\<^sub>2 ed e\<^sub>3 t)
+  then show ?case by auto
+next
+  case (BinAOp \<Gamma> e\<^sub>1 aop e\<^sub>2 sz t)
+  then show ?case sorry
+next
+  case (BinLOp \<Gamma> e\<^sub>1 lop e\<^sub>2 sz t)
+  then show ?case sorry
+next
+  case (UOp \<Gamma> uop e sz t)
+  then show ?case sorry
+next
+  case (UnsignedCast \<Gamma> e sz sz' t)
+  then show ?case sorry
+next
+  case (SignedCast \<Gamma> e sz sz' t)
+  then show ?case sorry
+next
+  case (HighCast \<Gamma> e sz sz' t)
+  then show ?case sorry
+next
+  case (LowCast \<Gamma> e sz sz' t)
+  then show ?case sorry
+next
+  case (Let \<Gamma> name t' e\<^sub>1 e\<^sub>2 t)
+  then show ?case sorry
+next
+  case (Ite \<Gamma> e\<^sub>1 e\<^sub>2 e\<^sub>3 t)
+  then show ?case sorry
+next
+  case (Extract \<Gamma> sz\<^sub>1 sz\<^sub>2 sz\<^sub>e\<^sub>x\<^sub>t\<^sub>r\<^sub>a\<^sub>c\<^sub>t sz e t)
+  then show ?case sorry
+next
+  case (Concat \<Gamma> e\<^sub>1 e\<^sub>2 sz\<^sub>c\<^sub>o\<^sub>n\<^sub>c\<^sub>a\<^sub>t sz\<^sub>1 sz\<^sub>2 t)
+  then show ?case 
+    apply (auto simp add: Let_def)
+    apply (cases \<open>eval_exp \<Delta> e\<^sub>1\<close>, auto)
+    apply (cases \<open>eval_exp \<Delta> e\<^sub>2\<close>, auto)
+    apply (cases
+    sledgehammer
+    sorry
+qed
+*)
 
 lemma \<Gamma>_exp_type_implies_type_t:
   assumes \<open>\<Gamma> \<turnstile> e :: t\<close>
       and \<open>(\<forall>var \<in> dom \<Delta>. snd var = type (the (\<Delta> var)))\<close>
     shows \<open>type (eval_exp \<Delta> e) = t\<close>
-  using assms apply (induct e)
-  apply (simp add: \<Gamma>_val_type_implies_type_t)
+using assms proof (induct rule: typing_expression_exp_induct)
+  case (Val \<Gamma> v t)
+  then show ?case 
+    using \<Gamma>_val_type_implies_type_t by force
+next
+  case (Var \<Gamma> name t)
+  then show ?case 
+    apply auto
+    by (metis domI option.sel snd_conv)
+next
+  case (Load \<Gamma> e\<^sub>1 e\<^sub>2 ed sz sz\<^sub>a\<^sub>d\<^sub>d\<^sub>r sz\<^sub>m\<^sub>e\<^sub>m t)
+  then show ?case 
+    apply (auto simp add: Let_def)
+    apply (cases \<open>eval_exp \<Delta> e\<^sub>1\<close>, auto)
+    apply (cases \<open>eval_exp \<Delta> e\<^sub>2\<close>, auto)
+    apply (subgoal_tac \<open>\<Gamma> \<turnstile> eval_exp \<Delta> e\<^sub>1 :: Mem (bits x32) sz\<^sub>m\<^sub>e\<^sub>m\<close>)
+    apply (subgoal_tac \<open>\<Gamma> \<turnstile> eval_exp \<Delta> e\<^sub>2 :: Imm (bits x32)\<close>)
+     apply auto
+    sledgehammer
+
+    by (meson XX \<Gamma>_val_type_implies_type_t typing_expression_exp.simps(2))
+    sorry
+next
+  case (Store \<Gamma> sz\<^sub>a\<^sub>d\<^sub>d\<^sub>r sz\<^sub>m\<^sub>e\<^sub>m sz\<^sub>v\<^sub>a\<^sub>l e\<^sub>1 e\<^sub>2 ed e\<^sub>3 t)
+  then show ?case sorry
+next
+  case (BinAOp \<Gamma> e\<^sub>1 aop e\<^sub>2 sz t)
+  then show ?case sorry
+next
+  case (BinLOp \<Gamma> e\<^sub>1 lop e\<^sub>2 sz t)
+  then show ?case sorry
+next
+  case (UOp \<Gamma> uop e sz t)
+  then show ?case sorry
+next
+  case (UnsignedCast \<Gamma> e sz sz' t)
+  then show ?case sorry
+next
+  case (SignedCast \<Gamma> e sz sz' t)
+  then show ?case sorry
+next
+  case (HighCast \<Gamma> e sz sz' t)
+  then show ?case sorry
+next
+  case (LowCast \<Gamma> e sz sz' t)
+  then show ?case sorry
+next
+  case (Let \<Gamma> name t' e\<^sub>1 e\<^sub>2 t)
+  then show ?case sorry
+next
+  case (Ite \<Gamma> e\<^sub>1 e\<^sub>2 e\<^sub>3 t)
+  then show ?case sorry
+next
+  case (Extract \<Gamma> sz\<^sub>1 sz\<^sub>2 sz\<^sub>e\<^sub>x\<^sub>t\<^sub>r\<^sub>a\<^sub>c\<^sub>t sz e t)
+  then show ?case sorry
+next
+  case (Concat \<Gamma> e\<^sub>1 e\<^sub>2 sz\<^sub>c\<^sub>o\<^sub>n\<^sub>c\<^sub>a\<^sub>t sz\<^sub>1 sz\<^sub>2 t)
+  then show ?case sorry
+qed
+  case (Val x)
+  then show ?case 
+    by (simp add: \<Gamma>_val_type_implies_type_t)
+next
+  case (Var x)
+  then show ?case
+    apply (cases x, auto)
+    by (metis domI option.sel snd_conv)
+next
+  case (Load e1 e2 x3 x4)
+  then show ?case 
+    sorry
+next
+  case (Store e1 e2 x3 x4 e3)
+  then show ?case sorry
+next
+  case (BinOp e1 x2a e2)
+  then show ?case
+    apply (cases t, auto)
+    apply (case_tac \<open>x2a\<close>, auto)
+    apply (case_tac \<open>eval_exp \<Delta> e1\<close>, auto)
+    apply (case_tac \<open>eval_exp \<Delta> e2\<close>, auto)
+    defer
+    apply (case_tac \<open>x1 = 1\<close>, auto)
+    defer
+    apply (metis old.nat.exhaust typing_expression_exp.simps(18) typing_expression_exp.simps(19))
+    defer
+    apply (case_tac \<open>eval_exp \<Delta> e1\<close>, auto)
+    apply (case_tac \<open>eval_exp \<Delta> e2\<close>, auto)
+
+    sorry
+next
+  case (UnOp x1a e)
+  then show ?case 
+    apply (cases t, auto)
+    apply (case_tac \<open>eval_exp \<Delta> e\<close>, auto)
+    sorry
+next
+  case (Cast x1a x2a e)
+  then show ?case 
+    apply (cases t, auto)
+    apply (case_tac x1a, auto)
+    apply (case_tac \<open>eval_exp \<Delta> e\<close>, auto)
+    defer
+    sledgehammer
+
+    sorry
+next
+  case (Let x1a e1 e2)
+  then show ?case sorry
+next
+  case (Ite e1 e2 e3)
+  then show ?case sorry
+next
+  case (Extract x1a x2a e)
+  then show ?case sorry
+next
+  case (Concat e1 e2)
+  then show ?case sorry
+qed
+
+
+  defer defer
+
+
+
+
+
   apply auto[1]
-  apply (metis domI option.sel snd_conv)
-  apply (induct t, simp_all)
+
+
+          
+          apply (induct t, simp_all)
   apply (auto simp add: Let_def)
   apply (case_tac \<open>type (eval_exp \<Delta> e1)\<close>)
   defer
@@ -411,7 +802,7 @@ lemma \<Gamma>_exp_type_implies_type_t:
   apply (case_tac \<open>eval_exp \<Delta> e2\<close>)
   apply auto
   oops
-
+*)
 
 lemma wf\<Delta>_birstep:
     fixes stmt :: stmt 
@@ -420,6 +811,7 @@ lemma wf\<Delta>_birstep:
       and \<open>(\<Delta>',w') = eval_stmt \<Delta> w stmt\<close>
     shows \<open>wf\<Delta> \<Delta>'\<close>
   using assms apply (cases stmt, auto)
+  apply (auto simp add: wf\<Delta>_def) 
      defer
   apply (case_tac \<open>eval_exp \<Delta> x2\<close>)
   apply auto
