Expression_Semantics.thy
@@ -9,142 +9,213 @@ where
   \<open>type (Immediate w) = Imm (bits w)\<close> | 
   \<open>type (Unknown str t) = t\<close>
 
-fun 
+definition 
   succ :: \<open>word \<Rightarrow> word\<close>
 where
   \<open>succ w\<^sub>1 = w\<^sub>1 +\<^sub>b\<^sub>v (1 \<Colon> bits w\<^sub>1)\<close>
 
 lemma SUCC: \<open>succ (num \<Colon> sz) = (num \<Colon> sz) +\<^sub>b\<^sub>v (1 \<Colon> sz)\<close>
-  by simp
+  by (simp add: succ_def)
 
-class expression =
-    fixes step :: \<open>variables \<Rightarrow> 'a \<Rightarrow> 'a\<close>  (infixl \<open>\<turnstile>\<close> 65)
-      and step_pred :: \<open>variables \<Rightarrow> 'a \<Rightarrow> 'a \<Rightarrow> bool\<close> (\<open>_ \<turnstile> _ \<leadsto> _\<close>)
+fun
+  load_val :: \<open>val \<Rightarrow> word \<Rightarrow> val\<close>
+where 
+  \<open>load_val (Storage v w v' _) w' = (if w = w' then v' else load_val v w')\<close> |
+  \<open>load_val (Unknown str (Mem _ sz)) _ = Unknown str (Imm sz)\<close>
 
-instantiation exp :: expression
-begin
-(* TODO REMOVE dummy cases *)
-fun 
-  step_exp :: \<open>variables \<Rightarrow> exp \<Rightarrow> exp\<close>
-where
-  \<open>step_exp \<Delta> (Val val) = (Val val)\<close> |
-  \<open>step_exp \<Delta> (Var var) = (let (name, t) = var in if var \<in> dom \<Delta> then (Val (the (\<Delta> var))) else (Val (Unknown [] t)))\<close> |
-  \<open>step_exp \<Delta> (Load e\<^sub>1 e\<^sub>2 ed sz) = (
-    case e\<^sub>2 of Val v\<^sub>2 \<Rightarrow> (
-      case e\<^sub>1 of Val v\<^sub>1 \<Rightarrow> (
-        case v\<^sub>1 of Storage v w\<^sub>1 v' sz' \<Rightarrow> (
-          case v\<^sub>2 of Immediate w\<^sub>2 \<Rightarrow> (
-            if sz > sz' then 
-              case ed of be \<Rightarrow> (Concat (Load (Val v\<^sub>1) (Val (Immediate w\<^sub>2)) be sz') ((Load (Val v\<^sub>1) (Val (Immediate (succ w\<^sub>2))) be (sz - sz'))))
-                | el \<Rightarrow> (Concat (Load (Val v\<^sub>1) (Val (Immediate (succ w\<^sub>2))) el (sz - sz')) ((Load (Val v\<^sub>1) (Val (Immediate w\<^sub>2)) el sz')))
-            else (
-              if w\<^sub>2 = w\<^sub>1 then (Val v')
-              else (Load (Val v) (Val (Immediate w\<^sub>2)) ed sz)
-            )
-          ) | Unknown str t \<Rightarrow> Val (Unknown str (Imm sz))
-        ) | Unknown str t \<Rightarrow> Val (Unknown str (Imm sz))
-      ) | _ \<Rightarrow> (Load (step_exp \<Delta> e\<^sub>1) (Val v\<^sub>2) ed sz)
-    ) | _ \<Rightarrow> (Load e\<^sub>1 (step_exp \<Delta> e\<^sub>2) ed sz)
-  )\<close> |
-  \<open>step_exp \<Delta> (Store e\<^sub>1 e\<^sub>2 ed sz e\<^sub>3) = (
-    case e\<^sub>3 of Val v\<^sub>3 \<Rightarrow> (
-      case e\<^sub>2 of Val v\<^sub>2 \<Rightarrow> (
-        case e\<^sub>1 of Val v\<^sub>1 \<Rightarrow> (
-          let t = type v\<^sub>1 in 
-          case v\<^sub>2 of Immediate w \<Rightarrow> (
-            case t of Mem _ sz' \<Rightarrow> (
-              if sz > sz' then 
-                case ed of be \<Rightarrow> (Store (Store (Val v\<^sub>1) (Val (Immediate w)) be sz' (Cast High sz' (Val v\<^sub>3))) (Val (Immediate (succ w))) be (sz - sz') (Cast Low (sz - sz') (Val v\<^sub>3)))
-                  | el \<Rightarrow> (Store (Store (Val v\<^sub>1) (Val (Immediate w)) el sz' (Cast Low sz' (Val v\<^sub>3))) (Val (Immediate (succ w))) el (sz - sz') (Cast High (sz - sz') (Val v\<^sub>3)))
-              else Val (Storage v\<^sub>1 w v\<^sub>3 sz')
-            )
-          ) | Unknown str t' \<Rightarrow> Val (Unknown str t)
-        ) | _ \<Rightarrow> (Store (step_exp \<Delta> e\<^sub>1) (Val v\<^sub>2) ed sz (Val v\<^sub>3))
-      ) | _ \<Rightarrow> (Store e\<^sub>1 (step_exp \<Delta> e\<^sub>2) ed sz (Val v\<^sub>3))
-    ) | _ \<Rightarrow> (Store e\<^sub>1 e\<^sub>2 ed sz (step_exp \<Delta> e\<^sub>3))
-  )\<close> |
-  \<open>step_exp \<Delta> (BinOp e\<^sub>1 binop e\<^sub>2) = (
-    case e\<^sub>1 of Val v\<^sub>1 \<Rightarrow> (
-      case e\<^sub>2 of Val v\<^sub>2 \<Rightarrow> (
-        case binop of
-          AOp aop \<Rightarrow> (case v\<^sub>1 of
-            Immediate w\<^sub>1 \<Rightarrow> (case v\<^sub>2 of 
-              Immediate w\<^sub>2 \<Rightarrow> Val (Immediate (operator_aop aop w\<^sub>1 w\<^sub>2)) |
-              Unknown str t \<Rightarrow> Val (Unknown str t)) |
-            Unknown str t \<Rightarrow> Val (Unknown str t))
-          |
-          LOp lop \<Rightarrow> (case v\<^sub>1 of
-            Immediate w\<^sub>1 \<Rightarrow> (case v\<^sub>2 of 
-              Immediate w\<^sub>2 \<Rightarrow> Val (Immediate (operator_lop lop w\<^sub>1 w\<^sub>2)) |
-              Unknown str t \<Rightarrow> Val (Unknown str (Imm 1))) |
-            Unknown str t \<Rightarrow> Val (Unknown str (Imm 1)))
-      ) | _ \<Rightarrow> (BinOp (Val v\<^sub>1) binop (step_exp \<Delta> e\<^sub>2))
-    ) | _ \<Rightarrow> (BinOp (step_exp \<Delta> e\<^sub>1) binop e\<^sub>2)
-  )\<close> |
-  \<open>step_exp \<Delta> (UnOp unop e) = (
-    case e of Val v \<Rightarrow> (
-      case v of Immediate w \<Rightarrow> Val (Immediate ((operator_unop unop) w))
-        | Unknown str t \<Rightarrow> Val (Unknown str t)
-    ) | _ \<Rightarrow> UnOp unop (step_exp \<Delta> e)
-  )\<close> |
-  \<open>step_exp \<Delta> (Cast cast sz e) = (
-    case e of Val v \<Rightarrow> (
-      case v of
-        Immediate w \<Rightarrow> (case cast of
-          Low \<Rightarrow> Val (Immediate (ext w \<sim> hi : (sz - 1) \<sim> lo : 0)) |
-          High \<Rightarrow> Val (Immediate (ext w \<sim> hi : (bits w - 1) \<sim> lo : (bits w - sz))) |
-          Signed \<Rightarrow> Val (Immediate (exts w \<sim> hi : (sz - 1) \<sim> lo : 0)) |
-          Unsigned \<Rightarrow> Val (Immediate (ext w \<sim> hi : (sz - 1) \<sim> lo : 0))) |
-        Unknown str t \<Rightarrow> Val (Unknown str (Imm sz))
-    ) | _ \<Rightarrow> Cast cast sz (step_exp \<Delta> e)
-  )\<close> |
-  \<open>step_exp \<Delta> (Let var e\<^sub>1 e\<^sub>2) = (
-    case e\<^sub>1 of Val v\<^sub>1 \<Rightarrow> (
-      [(Val v\<^sub>1)\<sslash>var]e\<^sub>2
-    ) | _ \<Rightarrow> Let var (step_exp \<Delta> e\<^sub>1) e\<^sub>2
-  )\<close> |
-  \<open>step_exp \<Delta> (Ite e\<^sub>1 e\<^sub>2 e\<^sub>3) = (
-    case e\<^sub>3 of Val v\<^sub>3 \<Rightarrow> (
-      case e\<^sub>2 of Val v\<^sub>2 \<Rightarrow> (
-        case e\<^sub>1 of Val v\<^sub>1 \<Rightarrow> (
-          case v\<^sub>1 of Immediate w \<Rightarrow> (
-            if w = true then Val v\<^sub>2
-            else Val v\<^sub>3
-          ) | Unknown str t \<Rightarrow> Val (Unknown str (type v\<^sub>2))
-        ) | _ \<Rightarrow> (Ite (step_exp \<Delta> e\<^sub>1) (Val v\<^sub>2) (Val v\<^sub>3))
-      ) | _ \<Rightarrow> (Ite e\<^sub>1 (step_exp \<Delta> e\<^sub>2) (Val v\<^sub>3))
-    ) | _ \<Rightarrow> (Ite e\<^sub>1 e\<^sub>2 (step_exp \<Delta> e\<^sub>3))
-  )\<close> |
-  \<open>step_exp \<Delta> (Extract sz\<^sub>1 sz\<^sub>2 e) = (
-    case e of Val v \<Rightarrow> (
-      case v of Immediate w \<Rightarrow> Val (Immediate (ext w \<sim> hi : sz\<^sub>1 \<sim> lo : sz\<^sub>2))
-        | Unknown str t \<Rightarrow> Val (Unknown str (Imm ((sz\<^sub>1 - sz\<^sub>2) + 1)))
-    ) | _ \<Rightarrow> Extract sz\<^sub>1 sz\<^sub>2 (step_exp \<Delta> e)
-  )\<close> |
-  \<open>step_exp \<Delta> (Concat e\<^sub>1 e\<^sub>2) = (
-    case e\<^sub>2 of Val v\<^sub>2 \<Rightarrow> (
-      case e\<^sub>1 of Val v\<^sub>1 \<Rightarrow> (
-        case v\<^sub>1 of
-          Immediate w\<^sub>1 \<Rightarrow> (case v\<^sub>2 of 
-            Immediate w\<^sub>2 \<Rightarrow> Val (Immediate (w\<^sub>1 \<cdot> w\<^sub>2)) |
-            Unknown str (Imm sz\<^sub>2) \<Rightarrow> case type v\<^sub>1 of
-              Imm sz\<^sub>1 \<Rightarrow> Val (Unknown str (Imm (sz\<^sub>1 + sz\<^sub>2)))
-          ) |
-          Unknown str (Imm sz\<^sub>1) \<Rightarrow> case type v\<^sub>2 of
-            Imm sz\<^sub>2 \<Rightarrow> Val (Unknown str (Imm (sz\<^sub>1 + sz\<^sub>2)))
-      ) | _ \<Rightarrow> (Concat (step_exp \<Delta> e\<^sub>1) (Val v\<^sub>2))
-    ) | _ \<Rightarrow> (Concat e\<^sub>1 (step_exp \<Delta> e\<^sub>2))
+lemma load_val_next: 
+  assumes \<open>w \<noteq> w'\<close>
+    shows \<open>load_val (Storage v w v' sz) w' = load_val v w'\<close>
+  using assms by auto
+
+fun
+  load_val_be :: \<open>val \<Rightarrow> word \<Rightarrow> nat \<Rightarrow> val\<close>
+where 
+  \<open>load_val_be mem w 0 = load_val mem w\<close> |
+  \<open>load_val_be mem w (Suc n) = (
+    case load_val_be mem (succ w) n of Immediate w\<^sub>c\<^sub>o\<^sub>n\<^sub>c\<^sub>a\<^sub>t \<Rightarrow> (
+      case load_val mem w of Immediate w\<^sub>v\<^sub>a\<^sub>l \<Rightarrow> Immediate (w\<^sub>v\<^sub>a\<^sub>l \<cdot> w\<^sub>c\<^sub>o\<^sub>n\<^sub>c\<^sub>a\<^sub>t)
+      | Unknown str (Imm sz) \<Rightarrow> Unknown str (Imm (bits w\<^sub>c\<^sub>o\<^sub>n\<^sub>c\<^sub>a\<^sub>t + sz)))
+    | Unknown str (Imm sz) \<Rightarrow> Unknown str (Imm sz)
   )\<close>
 
 fun
-  step_pred_exp :: \<open>variables \<Rightarrow> exp \<Rightarrow> exp \<Rightarrow> bool\<close>
+  load_val_el :: \<open>val \<Rightarrow> word \<Rightarrow> nat \<Rightarrow> val\<close>
+where 
+  \<open>load_val_el mem w 0 = load_val mem w\<close> |
+  \<open>load_val_el mem w (Suc n) = (
+    case load_val_el mem (succ w) n of Immediate w\<^sub>c\<^sub>o\<^sub>n\<^sub>c\<^sub>a\<^sub>t \<Rightarrow> (
+      case load_val mem w of Immediate w\<^sub>v\<^sub>a\<^sub>l \<Rightarrow> Immediate (w\<^sub>c\<^sub>o\<^sub>n\<^sub>c\<^sub>a\<^sub>t \<cdot> w\<^sub>v\<^sub>a\<^sub>l)
+      | v \<Rightarrow> v)
+    | v \<Rightarrow> v
+  )\<close>
+
+fun
+  load_val_en :: \<open>val \<Rightarrow> nat \<Rightarrow> word \<Rightarrow> nat \<Rightarrow> Endian \<Rightarrow> val\<close>
+where 
+  \<open>load_val_en mem sz\<^sub>m\<^sub>e\<^sub>m w sz\<^sub>v\<^sub>a\<^sub>l be =
+    load_val_be mem w (sz\<^sub>v\<^sub>a\<^sub>l div sz\<^sub>m\<^sub>e\<^sub>m - 1)
+  \<close> |
+  \<open>load_val_en mem sz\<^sub>m\<^sub>e\<^sub>m w sz\<^sub>v\<^sub>a\<^sub>l el =
+    load_val_el mem w (sz\<^sub>v\<^sub>a\<^sub>l div sz\<^sub>m\<^sub>e\<^sub>m - 1)\<close>
+
+definition
+  store_val :: \<open>val \<Rightarrow> word \<Rightarrow> val \<Rightarrow> nat \<Rightarrow> val\<close>
+where 
+  \<open>store_val mem w v sz\<^sub>m\<^sub>e\<^sub>m = Storage mem w v sz\<^sub>m\<^sub>e\<^sub>m\<close>
+
+fun
+  store_val_be :: \<open>val \<Rightarrow> nat \<Rightarrow> word \<Rightarrow> val \<Rightarrow> nat \<Rightarrow> val\<close>
+where 
+  \<open>store_val_be mem sz\<^sub>m\<^sub>e\<^sub>m w\<^sub>a\<^sub>d\<^sub>d\<^sub>r v\<^sub>v\<^sub>a\<^sub>l sz\<^sub>v\<^sub>a\<^sub>l = (
+    if sz\<^sub>m\<^sub>e\<^sub>m > 0 \<and> sz\<^sub>v\<^sub>a\<^sub>l > sz\<^sub>m\<^sub>e\<^sub>m then
+      let sz\<^sub>v\<^sub>a\<^sub>l' :: nat = (sz\<^sub>v\<^sub>a\<^sub>l - sz\<^sub>m\<^sub>e\<^sub>m) in 
+      let w\<^sub>a\<^sub>d\<^sub>d\<^sub>r' :: word = succ w\<^sub>a\<^sub>d\<^sub>d\<^sub>r in
+      case v\<^sub>v\<^sub>a\<^sub>l of Immediate w\<^sub>v\<^sub>a\<^sub>l \<Rightarrow> (
+        let w\<^sub>v\<^sub>a\<^sub>l\<^sub>_\<^sub>c\<^sub>o\<^sub>n\<^sub>c\<^sub>a\<^sub>t :: word = ext w\<^sub>v\<^sub>a\<^sub>l \<sim> hi : sz\<^sub>v\<^sub>a\<^sub>l' \<sim> lo : 0 in
+        let w\<^sub>v\<^sub>a\<^sub>l\<^sub>_\<^sub>v\<^sub>a\<^sub>l :: word = ext w\<^sub>v\<^sub>a\<^sub>l \<sim> hi : sz\<^sub>v\<^sub>a\<^sub>l \<sim> lo : sz\<^sub>v\<^sub>a\<^sub>l' in
+        let mem' :: val = store_val_be mem sz\<^sub>m\<^sub>e\<^sub>m w\<^sub>a\<^sub>d\<^sub>d\<^sub>r' (Immediate w\<^sub>v\<^sub>a\<^sub>l\<^sub>_\<^sub>c\<^sub>o\<^sub>n\<^sub>c\<^sub>a\<^sub>t) sz\<^sub>v\<^sub>a\<^sub>l' in
+          (store_val mem' w\<^sub>a\<^sub>d\<^sub>d\<^sub>r (Immediate w\<^sub>v\<^sub>a\<^sub>l\<^sub>_\<^sub>v\<^sub>a\<^sub>l) sz\<^sub>m\<^sub>e\<^sub>m)
+      ) | Unknown str t \<Rightarrow> (
+        let mem' :: val = store_val_be mem sz\<^sub>m\<^sub>e\<^sub>m w\<^sub>a\<^sub>d\<^sub>d\<^sub>r' (Unknown str (Imm sz\<^sub>v\<^sub>a\<^sub>l')) sz\<^sub>v\<^sub>a\<^sub>l' in
+          (store_val mem' w\<^sub>a\<^sub>d\<^sub>d\<^sub>r (Unknown str (Imm sz\<^sub>m\<^sub>e\<^sub>m)) sz\<^sub>m\<^sub>e\<^sub>m)
+      )
+    else
+      store_val mem w\<^sub>a\<^sub>d\<^sub>d\<^sub>r v\<^sub>v\<^sub>a\<^sub>l sz\<^sub>m\<^sub>e\<^sub>m
+  )\<close>
+
+fun
+  store_val_el :: \<open>val \<Rightarrow> nat \<Rightarrow> word \<Rightarrow> val \<Rightarrow> nat \<Rightarrow> val\<close>
+where 
+  \<open>store_val_el mem sz\<^sub>m\<^sub>e\<^sub>m w\<^sub>a\<^sub>d\<^sub>d\<^sub>r v\<^sub>v\<^sub>a\<^sub>l sz\<^sub>v\<^sub>a\<^sub>l = (
+    if sz\<^sub>m\<^sub>e\<^sub>m > 0 \<and> sz\<^sub>v\<^sub>a\<^sub>l > sz\<^sub>m\<^sub>e\<^sub>m then
+      let sz\<^sub>v\<^sub>a\<^sub>l' :: nat = (sz\<^sub>v\<^sub>a\<^sub>l - sz\<^sub>m\<^sub>e\<^sub>m) in
+      let w\<^sub>a\<^sub>d\<^sub>d\<^sub>r' :: word = succ w\<^sub>a\<^sub>d\<^sub>d\<^sub>r in
+      case v\<^sub>v\<^sub>a\<^sub>l of Immediate w\<^sub>v\<^sub>a\<^sub>l \<Rightarrow> (
+        let w\<^sub>v\<^sub>a\<^sub>l\<^sub>_\<^sub>c\<^sub>o\<^sub>n\<^sub>c\<^sub>a\<^sub>t :: word = ext w\<^sub>v\<^sub>a\<^sub>l \<sim> hi : sz\<^sub>v\<^sub>a\<^sub>l \<sim> lo : sz\<^sub>m\<^sub>e\<^sub>m in
+        let w\<^sub>v\<^sub>a\<^sub>l\<^sub>_\<^sub>v\<^sub>a\<^sub>l :: word = ext w\<^sub>v\<^sub>a\<^sub>l \<sim> hi : sz\<^sub>m\<^sub>e\<^sub>m \<sim> lo : 0 in
+        let mem' :: val = store_val_el mem sz\<^sub>m\<^sub>e\<^sub>m w\<^sub>a\<^sub>d\<^sub>d\<^sub>r' (Immediate w\<^sub>v\<^sub>a\<^sub>l\<^sub>_\<^sub>c\<^sub>o\<^sub>n\<^sub>c\<^sub>a\<^sub>t) sz\<^sub>v\<^sub>a\<^sub>l' in
+          (store_val mem' w\<^sub>a\<^sub>d\<^sub>d\<^sub>r (Immediate w\<^sub>v\<^sub>a\<^sub>l\<^sub>_\<^sub>v\<^sub>a\<^sub>l) sz\<^sub>m\<^sub>e\<^sub>m)
+      ) | Unknown str t \<Rightarrow> (
+        let mem' :: val = store_val_be mem sz\<^sub>m\<^sub>e\<^sub>m w\<^sub>a\<^sub>d\<^sub>d\<^sub>r' (Unknown str (Imm sz\<^sub>v\<^sub>a\<^sub>l')) sz\<^sub>v\<^sub>a\<^sub>l' in
+          (store_val mem' w\<^sub>a\<^sub>d\<^sub>d\<^sub>r (Unknown str (Imm sz\<^sub>m\<^sub>e\<^sub>m)) sz\<^sub>m\<^sub>e\<^sub>m)
+      )
+    else 
+      store_val mem w\<^sub>a\<^sub>d\<^sub>d\<^sub>r v\<^sub>v\<^sub>a\<^sub>l sz\<^sub>m\<^sub>e\<^sub>m
+  )\<close>
+
+fun
+  store_val_en :: \<open>val \<Rightarrow> nat \<Rightarrow> word \<Rightarrow> val \<Rightarrow> nat \<Rightarrow> Endian \<Rightarrow> val\<close>
+where 
+  \<open>store_val_en mem sz\<^sub>m\<^sub>e\<^sub>m w\<^sub>a\<^sub>d\<^sub>d\<^sub>r v\<^sub>v\<^sub>a\<^sub>l sz\<^sub>v\<^sub>a\<^sub>l be = store_val_be mem sz\<^sub>m\<^sub>e\<^sub>m w\<^sub>a\<^sub>d\<^sub>d\<^sub>r v\<^sub>v\<^sub>a\<^sub>l sz\<^sub>v\<^sub>a\<^sub>l\<close> |
+  \<open>store_val_en mem sz\<^sub>m\<^sub>e\<^sub>m w\<^sub>a\<^sub>d\<^sub>d\<^sub>r v\<^sub>v\<^sub>a\<^sub>l sz\<^sub>v\<^sub>a\<^sub>l el = store_val_el mem sz\<^sub>m\<^sub>e\<^sub>m w\<^sub>a\<^sub>d\<^sub>d\<^sub>r v\<^sub>v\<^sub>a\<^sub>l sz\<^sub>v\<^sub>a\<^sub>l\<close>
+ 
+
+function
+  eval_exp :: \<open>variables \<Rightarrow> exp \<Rightarrow> val\<close>
 where
-  \<open>step_pred_exp \<Delta> (Val val) e' = False\<close> |
-  \<open>step_pred_exp \<Delta> e e' = (e' = \<Delta> \<turnstile> e)\<close>
+  \<open>eval_exp \<Delta> (Val v) = v\<close> |
+  \<open>eval_exp \<Delta> (Var var) = (let (name, t) = var in if var \<in> dom \<Delta> then (the (\<Delta> var)) else (Unknown [] t))\<close> |
+  \<open>eval_exp \<Delta> (UnOp unop e) = ( 
+    case (eval_exp \<Delta> e) of
+      Immediate w \<Rightarrow> Immediate ((operator_unop unop) w) |
+      Unknown str t \<Rightarrow> Unknown str t
+  )\<close> |
+  \<open>eval_exp \<Delta> (BinOp e\<^sub>1 binop e\<^sub>2) = (
+    let v\<^sub>1 = (eval_exp \<Delta> e\<^sub>1) in
+    let v\<^sub>2 = (eval_exp \<Delta> e\<^sub>2) in
+    case binop of
+      AOp aop \<Rightarrow> (case v\<^sub>1 of
+        Immediate w\<^sub>1 \<Rightarrow> (case v\<^sub>2 of 
+          Immediate w\<^sub>2 \<Rightarrow> Immediate (operator_aop aop w\<^sub>1 w\<^sub>2) |
+          Unknown str t \<Rightarrow> Unknown str t) |
+        Unknown str t \<Rightarrow> Unknown str t)
+       |
+      LOp lop \<Rightarrow> (case v\<^sub>1 of
+        Immediate w\<^sub>1 \<Rightarrow> (case v\<^sub>2 of 
+          Immediate w\<^sub>2 \<Rightarrow> Immediate (operator_lop lop w\<^sub>1 w\<^sub>2) |
+          Unknown str t \<Rightarrow> Unknown str (Imm 1)) |
+        Unknown str t \<Rightarrow> Unknown str (Imm 1))
+  )\<close> |
+  \<open>eval_exp \<Delta> (Cast cast sz e) = (
+    let v = eval_exp \<Delta> e in
+    case v of
+      Immediate w \<Rightarrow> (case cast of
+        Low \<Rightarrow> Immediate (ext w \<sim> hi : (sz - 1) \<sim> lo : 0) |
+        High \<Rightarrow> Immediate (ext w \<sim> hi : (bits w - 1) \<sim> lo : (bits w - sz)) |
+        Signed \<Rightarrow> Immediate (exts w \<sim> hi : (sz - 1) \<sim> lo : 0) |
+        Unsigned \<Rightarrow> Immediate (ext w \<sim> hi : (sz - 1) \<sim> lo : 0)) |
+      Unknown str t \<Rightarrow> Unknown str (Imm sz)
+  )\<close> |
+  \<open>eval_exp \<Delta> (Let var e\<^sub>1 e\<^sub>2) = (eval_exp \<Delta> ([(eval_exp \<Delta> e\<^sub>1)\<sslash>var] e\<^sub>2))\<close> |
+  \<open>eval_exp \<Delta> (Ite e\<^sub>1 e\<^sub>2 e\<^sub>3) = (
+    let v\<^sub>1 = eval_exp \<Delta> e\<^sub>1 in
+    let v\<^sub>2 = eval_exp \<Delta> e\<^sub>2 in
+    case v\<^sub>1 of
+      Immediate w \<Rightarrow> (
+        if w = true then v\<^sub>2
+        else eval_exp \<Delta> e\<^sub>3) |
+      Unknown str t \<Rightarrow> Unknown str (type v\<^sub>2)
+  )\<close> |
+  \<open>eval_exp \<Delta> (Extract sz\<^sub>1 sz\<^sub>2 e) = (
+    case (eval_exp \<Delta> e) of
+      Immediate w \<Rightarrow> Immediate (ext w \<sim> hi : sz\<^sub>1 \<sim> lo : sz\<^sub>2) |
+      Unknown str t \<Rightarrow> Unknown str (Imm ((sz\<^sub>1 - sz\<^sub>2) + 1))
+  )\<close> |
+  \<open>eval_exp \<Delta> (Concat e\<^sub>1 e\<^sub>2) = (
+    let v\<^sub>1 = (eval_exp \<Delta> e\<^sub>1) in
+    let v\<^sub>2 = (eval_exp \<Delta> e\<^sub>2) in
+    case v\<^sub>1 of
+      Immediate w\<^sub>1 \<Rightarrow> (case v\<^sub>2 of 
+        Immediate w\<^sub>2 \<Rightarrow> Immediate (w\<^sub>1 \<cdot> w\<^sub>2) |
+        Unknown str (Imm sz\<^sub>2) \<Rightarrow> case type v\<^sub>1 of
+          Imm sz\<^sub>1 \<Rightarrow> Unknown str (Imm (sz\<^sub>1 + sz\<^sub>2))        
+      ) |
+      Unknown str (Imm sz\<^sub>1) \<Rightarrow> case type v\<^sub>2 of
+        Imm sz\<^sub>2 \<Rightarrow> Unknown str (Imm (sz\<^sub>1 + sz\<^sub>2))
+      
+  )\<close> |
+  \<open>eval_exp \<Delta> (Load e\<^sub>1 e\<^sub>2 ed sz\<^sub>v\<^sub>a\<^sub>l) = (
+    let v\<^sub>2 = eval_exp \<Delta> e\<^sub>2 in
+    let v\<^sub>1 = eval_exp \<Delta> e\<^sub>1 in 
+    case v\<^sub>1 of Storage v w v' sz\<^sub>m\<^sub>e\<^sub>m \<Rightarrow> (
+      case v\<^sub>2 of Immediate w\<^sub>a\<^sub>d\<^sub>d\<^sub>r \<Rightarrow> (
+        load_val_en v\<^sub>1 sz\<^sub>m\<^sub>e\<^sub>m w\<^sub>a\<^sub>d\<^sub>d\<^sub>r sz\<^sub>v\<^sub>a\<^sub>l ed
+      ) | Unknown str _ \<Rightarrow> Unknown str (Imm sz\<^sub>v\<^sub>a\<^sub>l)
+    ) | Unknown str _ \<Rightarrow> Unknown str (Imm sz\<^sub>v\<^sub>a\<^sub>l)
+  )\<close> |
+  \<open>eval_exp \<Delta> (Store e\<^sub>1 e\<^sub>2 ed sz\<^sub>v\<^sub>a\<^sub>l e\<^sub>3) = (
+    let v\<^sub>3 = eval_exp \<Delta> e\<^sub>3 in
+    let v\<^sub>2 = eval_exp \<Delta> e\<^sub>2 in 
+    let v\<^sub>1 = eval_exp \<Delta> e\<^sub>1 in
+    let t = type v\<^sub>1 in
+    case v\<^sub>2 of Immediate w\<^sub>a\<^sub>d\<^sub>d\<^sub>r \<Rightarrow> (
+      case t of Mem _ sz\<^sub>m\<^sub>e\<^sub>m \<Rightarrow> (
+        store_val_en v\<^sub>1 sz\<^sub>m\<^sub>e\<^sub>m w\<^sub>a\<^sub>d\<^sub>d\<^sub>r v\<^sub>3 sz\<^sub>v\<^sub>a\<^sub>l ed)
+    ) | Unknown str _ \<Rightarrow> Unknown str t
+  )\<close>
+  apply auto
+  by (metis old.prod.exhaust wfe.cases)
 
-instance ..
+lemma let_substitute_Let_size_less: 
+    \<open>size_class.size (Let var e\<^sub>1 e\<^sub>2) > size_class.size ([(eval_exp \<Delta> e\<^sub>1)\<sslash>var] e\<^sub>2)\<close>
+  apply auto
+  apply (induct e\<^sub>1, auto)
+  apply (induct e\<^sub>2, auto)
+  apply (metis add.commute add_less_mono add_mono_thms_linordered_field(1) less_Suc_eq)
+  using less_Suc_eq let_substitute_val_size_eq by presburger+
 
-end
+termination eval_exp
+  apply (relation \<open>(\<lambda>p. size_class.size (snd p)) <*mlex*> {}\<close>)
+  apply (auto simp add: wf_mlex mlex_prod_def)
+  using let_substitute_Let_size_less by simp
+
+fun 
+  step_pred_exp :: \<open>variables \<Rightarrow> exp \<Rightarrow> exp \<Rightarrow> bool\<close> (\<open>_ \<turnstile> _ \<leadsto> _\<close>)
+where
+  \<open>(_ \<turnstile> (Val v) \<leadsto> _) = False\<close> |
+  \<open>(\<Delta> \<turnstile> e \<leadsto> e') = (eval_exp \<Delta> e = eval_exp \<Delta> e')\<close>
+
 
 lemma VAL_NO_STEP: \<open>\<not>(\<Delta> \<turnstile> (Val v) \<leadsto> e')\<close>
   by simp
@@ -166,43 +237,51 @@ lemma VAR_UNKNOWN:
 
 lemma LOAD_STEP_ADDR:
   assumes \<open>(\<Delta> \<turnstile> e\<^sub>2 \<leadsto> e\<^sub>2')\<close>
-    shows \<open>\<Delta> \<turnstile> (Load e\<^sub>1 e\<^sub>2 ed sz) \<leadsto> (Load e\<^sub>1 e\<^sub>2' ed sz)\<close>
-  using assms by (cases e\<^sub>2, auto) 
+    shows \<open>\<Delta> \<turnstile> (Load e\<^sub>1 e\<^sub>2 ed sz) \<leadsto> (Load e\<^sub>1 e\<^sub>2' ed sz)\<close>  
+  using assms by (cases e\<^sub>2, auto)
 
 lemma LOAD_STEP_MEM:
   assumes \<open>(\<Delta> \<turnstile> e\<^sub>1 \<leadsto> e\<^sub>1')\<close>
     shows \<open>\<Delta> \<turnstile> (Load e\<^sub>1 (Val v\<^sub>2) ed sz) \<leadsto> (Load e\<^sub>1' (Val v\<^sub>2) ed sz)\<close>
   using assms by (cases e\<^sub>1, auto)
 
-lemma LOAD_BYTE: \<open>\<Delta> \<turnstile> (Load (Val (Storage v w v' sz)) (Val (Immediate w)) ed' sz) \<leadsto> (Val v')\<close>
-  by auto
+lemma LOAD_BYTE: 
+  assumes \<open>sz \<noteq> 0\<close> 
+    shows \<open>\<Delta> \<turnstile> (Load (Val (Storage v w v' sz)) (Val (Immediate w)) ed sz) \<leadsto> (Val v')\<close>
+  using assms by (cases ed, auto)
 
 lemma LOAD_BYTE_FROM_NEXT:
-  assumes \<open>w\<^sub>1 \<noteq> w\<^sub>2\<close>
+  assumes \<open>w\<^sub>1 \<noteq> w\<^sub>2\<close> and \<open>sz \<noteq> 0\<close> and \<open>type v = Mem (bits w\<^sub>1) sz\<close> (*wf can prove this*)
     shows \<open>\<Delta> \<turnstile> (Load (Val (Storage v w\<^sub>1 v' sz)) (Val (Immediate w\<^sub>2)) ed sz) \<leadsto> (Load (Val v) (Val (Immediate w\<^sub>2)) ed sz)\<close>
-  using assms by auto
+  using assms apply auto
+  apply (cases ed, auto)
+  by (cases v, auto)+
 
 lemma LOAD_UN_MEM: \<open>\<Delta> \<turnstile> (Load (Val (Unknown str t)) (Val v) ed sz) \<leadsto> (Val (Unknown str (Imm sz)))\<close>
-  by auto
+  by (auto simp add: Let_def)
 
 lemma LOAD_UN_ADDR: \<open>\<Delta> \<turnstile> (Load (Val (Storage v w\<^sub>1 v' sz)) (Val (Unknown str t)) ed sz') \<leadsto> (Val (Unknown str (Imm sz')))\<close>
   by auto
 
 lemma LOAD_WORD_BE:
-  assumes \<open>sz' > sz\<close> and \<open>succ w = w'\<close> and \<open>v = (Storage v' w'' v'' sz)\<close> 
+  assumes \<open>sz' > sz\<close> and \<open>sz \<noteq> 0\<close> and \<open>succ w = w'\<close> and \<open>type v = (Mem sasas sz)\<close> 
     shows \<open>\<Delta> \<turnstile> (Load (Val v) (Val (Immediate w)) be sz') \<leadsto> (Concat (Load (Val v) (Val (Immediate w)) be sz) ((Load (Val v) (Val (Immediate w')) be (sz' - sz))))\<close> 
-  using assms by auto
+  apply (auto simp only: step_pred_exp.simps eval_exp.simps Let_def)
+  apply (cases v, auto)
+  using assms(4) apply auto
+  apply (metis Suc_leD Suc_leI assms(1) le_add_diff_inverse)
+  oops
+
 
 lemma LOAD_WORD_EL:
-  assumes \<open>sz' > sz\<close> and \<open>succ w = w'\<close> and \<open>v = (Storage v' w'' v'' sz)\<close>
+  assumes \<open>sz' > sz\<close> and \<open>sz \<noteq> 0\<close> and \<open>succ w = w'\<close> and \<open>v = (Storage v' w'' v'' sz)\<close>
     shows \<open>\<Delta> \<turnstile> (Load (Val v) (Val (Immediate w)) el sz') \<leadsto> (Concat (Load (Val v) (Val (Immediate w')) el (sz' - sz)) ((Load (Val v) (Val (Immediate w)) el sz)))\<close> 
-  using assms by auto
-
+  oops
 
 lemma STORE_STEP_VAL:
   assumes \<open>\<Delta> \<turnstile> e\<^sub>3 \<leadsto> e\<^sub>3'\<close>
     shows \<open>\<Delta> \<turnstile> (Store e\<^sub>1 e\<^sub>2 ed sz e\<^sub>3) \<leadsto> (Store e\<^sub>1 e\<^sub>2 ed sz e\<^sub>3')\<close> 
-  using assms by (cases e\<^sub>3, auto) 
+  using assms by (cases e\<^sub>3, auto)
 
 lemma STORE_STEP_ADDR:
   assumes \<open>\<Delta> \<turnstile> e\<^sub>2 \<leadsto> e\<^sub>2'\<close>
@@ -215,26 +294,30 @@ lemma STORE_STEP_MEM:
   using assms by (cases e\<^sub>1, auto) 
 
 lemma STORE_WORD_BE:
-  assumes \<open>sz' > sz\<close> and \<open>succ w = w'\<close> and \<open>type v = (Mem sz\<^sub>m\<^sub>e\<^sub>m sz)\<close> 
+  assumes \<open>sz' > sz\<close> and \<open>succ w = w'\<close> and \<open>type v = Mem sz\<^sub>a\<^sub>d\<^sub>d\<^sub>r sz\<^sub>m\<^sub>e\<^sub>m\<close> 
       and \<open>e\<^sub>1 = (Store (Val v) (Val (Immediate w)) be sz (Cast High sz (Val val)))\<close>
     shows \<open>\<Delta> \<turnstile> (Store (Val v) (Val (Immediate w)) be sz' (Val val)) \<leadsto> (Store e\<^sub>1 (Val (Immediate w')) be (sz' - sz) (Cast Low (sz' - sz) (Val val)))\<close> 
-  using assms by auto
+  oops
 
 lemma STORE_WORD_EL:
-  assumes \<open>sz' > sz\<close> and \<open>succ w = w'\<close> and \<open>type v = (Mem sz\<^sub>m\<^sub>e\<^sub>m sz)\<close> 
-      and \<open>e\<^sub>1 = (Store (Val v) (Val (Immediate w)) el sz (Cast Low sz (Val val)))\<close>
-    shows \<open>\<Delta> \<turnstile> (Store (Val v) (Val (Immediate w)) el sz' (Val val)) \<leadsto> (Store e\<^sub>1 (Val (Immediate w')) el (sz' - sz) (Cast High (sz' - sz) (Val val)))\<close>
-  using assms by auto
+  assumes \<open>sz' > sz\<^sub>m\<^sub>e\<^sub>m\<close> and \<open>sz\<^sub>m\<^sub>e\<^sub>m > 0\<close> and \<open>succ w = w'\<close> and \<open>type v = Mem sz\<^sub>a\<^sub>d\<^sub>d\<^sub>r sz\<^sub>m\<^sub>e\<^sub>m\<close> 
+      and \<open>e\<^sub>1 = (Store (Val v) (Val (Immediate w)) el sz\<^sub>m\<^sub>e\<^sub>m (Cast Low sz\<^sub>m\<^sub>e\<^sub>m (Val val)))\<close>
+    shows \<open>\<Delta> \<turnstile> (Store (Val v) (Val (Immediate w)) el sz' (Val val)) \<leadsto> (Store e\<^sub>1 (Val (Immediate w')) el (sz' - sz\<^sub>m\<^sub>e\<^sub>m) (Cast High (sz' - sz\<^sub>m\<^sub>e\<^sub>m) (Val val)))\<close>
+  oops
 
 lemma STORE_VAL:
-  assumes \<open>type v = Mem sz\<^sub>m\<^sub>e\<^sub>m sz\<close>
-    shows \<open>\<Delta> \<turnstile> (Store (Val v) (Val (Immediate w)) ed sz (Val v')) \<leadsto> (Val (Storage v w v' sz))\<close>
-  using assms by auto
+  assumes \<open>type v = Mem sz\<^sub>a\<^sub>d\<^sub>d\<^sub>r sz\<^sub>m\<^sub>e\<^sub>m\<close>
+    shows \<open>\<Delta> \<turnstile> (Store (Val v) (Val (Immediate w)) ed sz\<^sub>m\<^sub>e\<^sub>m (Val v')) \<leadsto> (Val (Storage v w v' sz\<^sub>m\<^sub>e\<^sub>m))\<close>
+  using assms apply (cases ed, auto)
+  by (auto simp add: store_val_def)
+
+
 
 lemma STORE_UN_ADDR:
   assumes \<open>type v = t\<close>
     shows \<open>\<Delta> \<turnstile> (Store (Val v) (Val (Unknown str t')) ed sz' (Val v')) \<leadsto> (Val (Unknown str t))\<close>
-  using assms by auto
+  using assms by (cases t, auto)
+ 
 
 lemma LET_STEP:
   assumes \<open>\<Delta> \<turnstile> e\<^sub>1 \<leadsto> e\<^sub>1'\<close>
@@ -242,7 +325,7 @@ lemma LET_STEP:
   using assms by (cases e\<^sub>1, auto)
 
 lemma LET: \<open>\<Delta> \<turnstile> (Let var (Val v\<^sub>1) e\<^sub>2) \<leadsto> ([(Val v\<^sub>1)\<sslash>var]e\<^sub>2)\<close>
-  by auto
+  by (simp add: let_substitue_val_exp_val_eq)
 
 lemma ITE_STEP_COND:
   assumes \<open>\<Delta> \<turnstile> e\<^sub>1 \<leadsto> e\<^sub>1'\<close>
@@ -257,7 +340,10 @@ lemma ITE_STEP_THEN:
 lemma ITE_STEP_ELSE:
   assumes \<open>\<Delta> \<turnstile> e\<^sub>3 \<leadsto> e\<^sub>3'\<close>
     shows \<open>\<Delta> \<turnstile> (Ite e\<^sub>1 e\<^sub>2 e\<^sub>3) \<leadsto> (Ite e\<^sub>1 e\<^sub>2 e\<^sub>3')\<close>
-  using assms by (cases e\<^sub>3, auto)
+  using assms apply (auto simp add: Let_def)
+  apply (cases \<open>eval_exp \<Delta> e\<^sub>1\<close>, auto)
+  by (cases e\<^sub>3, auto)
+  
 
 lemma ITE_TRUE: \<open>\<Delta> \<turnstile> (Ite (Val (Immediate true)) (Val v\<^sub>2) (Val v\<^sub>3)) \<leadsto> (Val v\<^sub>2)\<close>
   by auto
@@ -335,16 +421,16 @@ lemma EQ_SAME: \<open>\<Delta> \<turnstile> (BinOp (Val (Immediate w)) (LOp Eq) 
   by auto
 
 lemma EQ_DIFF: 
-  assumes \<open>w\<^sub>1 \<noteq> w\<^sub>2\<close>
+  assumes \<open>w\<^sub>1 \<noteq>\<^sub>b\<^sub>v w\<^sub>2 = true\<close>
+      and \<open>bits w\<^sub>1 = bits w\<^sub>2\<close>
     shows \<open>\<Delta> \<turnstile> (BinOp (Val (Immediate w\<^sub>1)) (LOp Eq) (Val (Immediate w\<^sub>2))) \<leadsto> (Val (Immediate false))\<close>
-  using assms apply auto
-  sorry
+  using assms by auto 
 
 lemma NEQ_SAME: \<open>\<Delta> \<turnstile> (BinOp (Val (Immediate w)) (LOp Neq) (Val (Immediate w))) \<leadsto> (Val (Immediate false))\<close>
   by auto
 
 lemma NEQ_DIFF: 
-  assumes \<open>w\<^sub>1 \<noteq> w\<^sub>2\<close>
+  assumes \<open>w\<^sub>1 \<noteq>\<^sub>b\<^sub>v w\<^sub>2 = true\<close>
     shows \<open>\<Delta> \<turnstile> (BinOp (Val (Immediate w\<^sub>1)) (LOp Neq) (Val (Immediate w\<^sub>2))) \<leadsto> (Val (Immediate true))\<close>
   using assms by auto
 
@@ -421,183 +507,6 @@ lemma CAST_UNSIGNED: \<open>\<Delta> \<turnstile> (Cast Unsigned sz (Val (Immedi
   by auto
 
 
-
-
-
-fun
-  load_val :: \<open>val \<Rightarrow> word \<Rightarrow> nat \<Rightarrow> val\<close>
-where 
-  \<open>load_val (Storage v w v' sz\<^sub>m\<^sub>e\<^sub>m) w' sz\<^sub>v\<^sub>a\<^sub>l = (if (w = w' \<and> sz\<^sub>m\<^sub>e\<^sub>m = sz\<^sub>v\<^sub>a\<^sub>l) then v' else load_val v w' sz\<^sub>v\<^sub>a\<^sub>l)\<close> |
-  \<open>load_val (Unknown str t) _ sz\<^sub>v\<^sub>a\<^sub>l = Unknown str (Imm sz\<^sub>v\<^sub>a\<^sub>l)\<close>
-
-fun
-  load_val_be :: \<open>val \<Rightarrow> nat \<Rightarrow> word \<Rightarrow> nat \<Rightarrow> val\<close>
-where 
-  \<open>load_val_be mem sz\<^sub>m\<^sub>e\<^sub>m w sz\<^sub>v\<^sub>a\<^sub>l = (
-    case load_val mem w sz\<^sub>m\<^sub>e\<^sub>m of
-      Immediate w\<^sub>v\<^sub>a\<^sub>l \<Rightarrow> (
-        if sz\<^sub>m\<^sub>e\<^sub>m > 0 \<and> sz\<^sub>v\<^sub>a\<^sub>l > sz\<^sub>m\<^sub>e\<^sub>m then
-          let sz\<^sub>v\<^sub>a\<^sub>l' = (sz\<^sub>v\<^sub>a\<^sub>l - sz\<^sub>m\<^sub>e\<^sub>m) in 
-          let w' = succ w in
-          case load_val_be mem sz\<^sub>m\<^sub>e\<^sub>m w' sz\<^sub>v\<^sub>a\<^sub>l' of
-            Immediate w\<^sub>c\<^sub>o\<^sub>n\<^sub>c\<^sub>a\<^sub>t \<Rightarrow> Immediate (w\<^sub>v\<^sub>a\<^sub>l \<cdot> w\<^sub>c\<^sub>o\<^sub>n\<^sub>c\<^sub>a\<^sub>t) |
-            Unknown str _ \<Rightarrow> Unknown str (Imm sz\<^sub>v\<^sub>a\<^sub>l)
-        else Immediate w\<^sub>v\<^sub>a\<^sub>l
-      ) |
-      Unknown str _ \<Rightarrow> Unknown str (Imm sz\<^sub>v\<^sub>a\<^sub>l)
-  )\<close>
-
-fun
-  load_val_el :: \<open>val \<Rightarrow> nat \<Rightarrow> word \<Rightarrow> nat \<Rightarrow> val\<close>
-where 
-  \<open>load_val_el mem sz\<^sub>m\<^sub>e\<^sub>m w sz\<^sub>v\<^sub>a\<^sub>l = (
-    case load_val mem w sz\<^sub>m\<^sub>e\<^sub>m of
-      Immediate w\<^sub>v\<^sub>a\<^sub>l \<Rightarrow> (
-        if sz\<^sub>m\<^sub>e\<^sub>m > 0 \<and> sz\<^sub>v\<^sub>a\<^sub>l > sz\<^sub>m\<^sub>e\<^sub>m then
-          let sz\<^sub>v\<^sub>a\<^sub>l' = (sz\<^sub>v\<^sub>a\<^sub>l - sz\<^sub>m\<^sub>e\<^sub>m) in 
-          let w' = succ w in
-          case load_val_el mem sz\<^sub>m\<^sub>e\<^sub>m w' sz\<^sub>v\<^sub>a\<^sub>l' of
-            Immediate w\<^sub>c\<^sub>o\<^sub>n\<^sub>c\<^sub>a\<^sub>t \<Rightarrow> Immediate (w\<^sub>c\<^sub>o\<^sub>n\<^sub>c\<^sub>a\<^sub>t \<cdot> w\<^sub>v\<^sub>a\<^sub>l) |
-            Unknown str _ \<Rightarrow> Unknown str (Imm sz\<^sub>v\<^sub>a\<^sub>l)
-        else Immediate w\<^sub>v\<^sub>a\<^sub>l
-      ) |
-      Unknown str _ \<Rightarrow> Unknown str (Imm sz\<^sub>v\<^sub>a\<^sub>l)
-  )\<close>
-
-fun
-  store_val :: \<open>val \<Rightarrow> word \<Rightarrow> val \<Rightarrow> nat \<Rightarrow> val\<close>
-where 
-  \<open>store_val (Storage mem w v _) w' v' sz\<^sub>m\<^sub>e\<^sub>m = (
-    let mem' = store_val mem w' v' sz\<^sub>m\<^sub>e\<^sub>m in
-    if w = w' then mem'
-    else (Storage mem' w v sz\<^sub>m\<^sub>e\<^sub>m)
-  )\<close> |
-  \<open>store_val mem w v sz\<^sub>m\<^sub>e\<^sub>m = Storage mem w v sz\<^sub>m\<^sub>e\<^sub>m\<close>
-
-fun
-  store_val_be :: \<open>val \<Rightarrow> nat \<Rightarrow> word \<Rightarrow> word \<Rightarrow> nat \<Rightarrow> val\<close>
-where 
-  \<open>store_val_be mem sz\<^sub>m\<^sub>e\<^sub>m w\<^sub>a\<^sub>d\<^sub>d\<^sub>r w\<^sub>v\<^sub>a\<^sub>l sz\<^sub>v\<^sub>a\<^sub>l = (
-    if sz\<^sub>m\<^sub>e\<^sub>m > 0 \<and> sz\<^sub>v\<^sub>a\<^sub>l > sz\<^sub>m\<^sub>e\<^sub>m then
-      let sz\<^sub>v\<^sub>a\<^sub>l' :: nat = (sz\<^sub>v\<^sub>a\<^sub>l - sz\<^sub>m\<^sub>e\<^sub>m) in 
-      let w\<^sub>v\<^sub>a\<^sub>l\<^sub>_\<^sub>c\<^sub>o\<^sub>n\<^sub>c\<^sub>a\<^sub>t :: word = ext w\<^sub>v\<^sub>a\<^sub>l \<sim> hi : sz\<^sub>v\<^sub>a\<^sub>l' \<sim> lo : 0 in
-      let w\<^sub>v\<^sub>a\<^sub>l\<^sub>_\<^sub>v\<^sub>a\<^sub>l :: word = ext w\<^sub>v\<^sub>a\<^sub>l \<sim> hi : sz\<^sub>v\<^sub>a\<^sub>l \<sim> lo : sz\<^sub>v\<^sub>a\<^sub>l' in
-      let w\<^sub>a\<^sub>d\<^sub>d\<^sub>r' :: word = succ w\<^sub>a\<^sub>d\<^sub>d\<^sub>r in
-      (store_val (store_val_be mem sz\<^sub>m\<^sub>e\<^sub>m w\<^sub>a\<^sub>d\<^sub>d\<^sub>r' w\<^sub>v\<^sub>a\<^sub>l\<^sub>_\<^sub>c\<^sub>o\<^sub>n\<^sub>c\<^sub>a\<^sub>t sz\<^sub>v\<^sub>a\<^sub>l') w\<^sub>a\<^sub>d\<^sub>d\<^sub>r (Immediate w\<^sub>v\<^sub>a\<^sub>l\<^sub>_\<^sub>v\<^sub>a\<^sub>l) sz\<^sub>m\<^sub>e\<^sub>m)
-    else
-      store_val mem w\<^sub>a\<^sub>d\<^sub>d\<^sub>r (Immediate w\<^sub>v\<^sub>a\<^sub>l) sz\<^sub>m\<^sub>e\<^sub>m
-  )\<close>
-
-fun
-  store_val_el :: \<open>val \<Rightarrow> nat \<Rightarrow> word \<Rightarrow> word \<Rightarrow> nat \<Rightarrow> val\<close>
-where 
-  \<open>store_val_el mem sz\<^sub>m\<^sub>e\<^sub>m w\<^sub>a\<^sub>d\<^sub>d\<^sub>r w\<^sub>v\<^sub>a\<^sub>l sz\<^sub>v\<^sub>a\<^sub>l = (
-    if sz\<^sub>m\<^sub>e\<^sub>m > 0 \<and> sz\<^sub>v\<^sub>a\<^sub>l > sz\<^sub>m\<^sub>e\<^sub>m then
-      let sz\<^sub>v\<^sub>a\<^sub>l' :: nat = (sz\<^sub>v\<^sub>a\<^sub>l - sz\<^sub>m\<^sub>e\<^sub>m) in 
-      let w\<^sub>v\<^sub>a\<^sub>l\<^sub>_\<^sub>c\<^sub>o\<^sub>n\<^sub>c\<^sub>a\<^sub>t :: word = ext w\<^sub>v\<^sub>a\<^sub>l \<sim> hi : sz\<^sub>v\<^sub>a\<^sub>l \<sim> lo : sz\<^sub>m\<^sub>e\<^sub>m in
-      let w\<^sub>v\<^sub>a\<^sub>l\<^sub>_\<^sub>v\<^sub>a\<^sub>l :: word = ext w\<^sub>v\<^sub>a\<^sub>l \<sim> hi : sz\<^sub>m\<^sub>e\<^sub>m \<sim> lo : 0 in
-      let w\<^sub>a\<^sub>d\<^sub>d\<^sub>r' :: word = succ w\<^sub>a\<^sub>d\<^sub>d\<^sub>r in
-      (store_val (store_val_el mem sz\<^sub>m\<^sub>e\<^sub>m w\<^sub>a\<^sub>d\<^sub>d\<^sub>r' w\<^sub>v\<^sub>a\<^sub>l\<^sub>_\<^sub>c\<^sub>o\<^sub>n\<^sub>c\<^sub>a\<^sub>t sz\<^sub>v\<^sub>a\<^sub>l') w\<^sub>a\<^sub>d\<^sub>d\<^sub>r (Immediate w\<^sub>v\<^sub>a\<^sub>l\<^sub>_\<^sub>v\<^sub>a\<^sub>l) sz\<^sub>m\<^sub>e\<^sub>m)
-    else 
-      store_val mem w\<^sub>a\<^sub>d\<^sub>d\<^sub>r (Immediate w\<^sub>v\<^sub>a\<^sub>l) sz\<^sub>m\<^sub>e\<^sub>m
-  )\<close>
-
-
-
-
-
-
-
-
-fun
-  eval_exp :: \<open>variables \<Rightarrow> exp \<Rightarrow> val\<close>
-where
-  \<open>eval_exp \<Delta> (Val v) = v\<close> |
-  \<open>eval_exp \<Delta> (Var var) = (let (name, t) = var in if var \<in> dom \<Delta> then (the (\<Delta> var)) else (Unknown [] t))\<close> |
-  \<open>eval_exp \<Delta> (UnOp unop e) = ( 
-    case (eval_exp \<Delta> e) of
-      Immediate w \<Rightarrow> Immediate ((operator_unop unop) w) |
-      Unknown str t \<Rightarrow> Unknown str t
-  )\<close> |
-  \<open>eval_exp \<Delta> (BinOp e\<^sub>1 binop e\<^sub>2) = (
-    let v\<^sub>1 = (eval_exp \<Delta> e\<^sub>1) in
-    let v\<^sub>2 = (eval_exp \<Delta> e\<^sub>2) in
-    case binop of
-      AOp aop \<Rightarrow> (case v\<^sub>1 of
-        Immediate w\<^sub>1 \<Rightarrow> (case v\<^sub>2 of 
-          Immediate w\<^sub>2 \<Rightarrow> Immediate (operator_aop aop w\<^sub>1 w\<^sub>2) |
-          Unknown str t \<Rightarrow> Unknown str t) |
-        Unknown str t \<Rightarrow> Unknown str t)
-       |
-      LOp lop \<Rightarrow> (case v\<^sub>1 of
-        Immediate w\<^sub>1 \<Rightarrow> (case v\<^sub>2 of 
-          Immediate w\<^sub>2 \<Rightarrow> Immediate (operator_lop lop w\<^sub>1 w\<^sub>2) |
-          Unknown str t \<Rightarrow> Unknown str (Imm 1)) |
-        Unknown str t \<Rightarrow> Unknown str (Imm 1))
-  )\<close> |
-  \<open>eval_exp \<Delta> (Cast cast sz e) = (
-    let v = eval_exp \<Delta> e in
-    case v of
-      Immediate w \<Rightarrow> (case cast of
-        Low \<Rightarrow> Immediate (ext w \<sim> hi : (sz - 1) \<sim> lo : 0) |
-        High \<Rightarrow> Immediate (ext w \<sim> hi : (bits w - 1) \<sim> lo : (bits w - sz)) |
-        Signed \<Rightarrow> Immediate (exts w \<sim> hi : (sz - 1) \<sim> lo : 0) |
-        Unsigned \<Rightarrow> Immediate (ext w \<sim> hi : (sz - 1) \<sim> lo : 0)) |
-      Unknown str t \<Rightarrow> Unknown str (Imm sz)
-  )\<close> |
-  \<open>eval_exp \<Delta> (Let var e\<^sub>1 e\<^sub>2) = (eval_exp (\<Delta>(var \<mapsto> (eval_exp \<Delta> e\<^sub>1))) e\<^sub>2)\<close> |
-  \<open>eval_exp \<Delta> (Ite e\<^sub>1 e\<^sub>2 e\<^sub>3) = (
-    let v\<^sub>1 = eval_exp \<Delta> e\<^sub>1 in
-    let v\<^sub>2 = eval_exp \<Delta> e\<^sub>2 in
-    case v\<^sub>1 of
-      Immediate w \<Rightarrow> (
-        if w = true then v\<^sub>2
-        else eval_exp \<Delta> e\<^sub>3) |
-      Unknown str t \<Rightarrow> Unknown str (type v\<^sub>2)
-  )\<close> |
-  \<open>eval_exp \<Delta> (Extract sz\<^sub>1 sz\<^sub>2 e) = (
-    case (eval_exp \<Delta> e) of
-      Immediate w \<Rightarrow> Immediate (ext w \<sim> hi : sz\<^sub>1 \<sim> lo : sz\<^sub>2) |
-      Unknown str t \<Rightarrow> Unknown str (Imm ((sz\<^sub>1 - sz\<^sub>2) + 1))
-  )\<close> |
-  \<open>eval_exp \<Delta> (Concat e\<^sub>1 e\<^sub>2) = (
-    let v\<^sub>1 = (eval_exp \<Delta> e\<^sub>1) in
-    let v\<^sub>2 = (eval_exp \<Delta> e\<^sub>2) in
-    case v\<^sub>1 of
-      Immediate w\<^sub>1 \<Rightarrow> (case v\<^sub>2 of 
-        Immediate w\<^sub>2 \<Rightarrow> Immediate (w\<^sub>1 \<cdot> w\<^sub>2) |
-        Unknown str (Imm sz\<^sub>2) \<Rightarrow> case type v\<^sub>1 of
-          Imm sz\<^sub>1 \<Rightarrow> Unknown str (Imm (sz\<^sub>1 + sz\<^sub>2))        
-      ) |
-      Unknown str (Imm sz\<^sub>1) \<Rightarrow> case type v\<^sub>2 of
-        Imm sz\<^sub>2 \<Rightarrow> Unknown str (Imm (sz\<^sub>1 + sz\<^sub>2))
-      
-  )\<close> |
-  \<open>eval_exp \<Delta> (Load e\<^sub>1 e\<^sub>2 ed sz\<^sub>v\<^sub>a\<^sub>l) = (
-    let v\<^sub>1 = eval_exp \<Delta> e\<^sub>1 in 
-    case type v\<^sub>1 of Mem _ sz\<^sub>m\<^sub>e\<^sub>m \<Rightarrow> (
-      case eval_exp \<Delta> e\<^sub>2 of 
-        Immediate w \<Rightarrow> (
-          case ed of
-            be \<Rightarrow> load_val_be v\<^sub>1 sz\<^sub>m\<^sub>e\<^sub>m w sz\<^sub>v\<^sub>a\<^sub>l |
-            el \<Rightarrow> load_val_el v\<^sub>1 sz\<^sub>m\<^sub>e\<^sub>m w sz\<^sub>v\<^sub>a\<^sub>l
-        ) |
-        Unknown str _ \<Rightarrow> Unknown str (Imm sz\<^sub>v\<^sub>a\<^sub>l)
-  ))\<close> |
-  \<open>eval_exp \<Delta> (Store e\<^sub>1 e\<^sub>2 ed sz\<^sub>v\<^sub>a\<^sub>l e\<^sub>3) = (
-    let v\<^sub>1 = eval_exp \<Delta> e\<^sub>1 in 
-    case type v\<^sub>1 of Mem _ sz\<^sub>m\<^sub>e\<^sub>m \<Rightarrow> (
-      case eval_exp \<Delta> e\<^sub>2 of 
-        Immediate w \<Rightarrow> (
-          case ed of
-            be \<Rightarrow> load_val_be v\<^sub>1 sz\<^sub>m\<^sub>e\<^sub>m w sz\<^sub>v\<^sub>a\<^sub>l |
-            el \<Rightarrow> load_val_el v\<^sub>1 sz\<^sub>m\<^sub>e\<^sub>m w sz\<^sub>v\<^sub>a\<^sub>l
-        ) |
-        Unknown str _ \<Rightarrow> Unknown str (Imm sz\<^sub>v\<^sub>a\<^sub>l)
-  ))\<close>
-
-
-
 fun
   eval_exps_pred :: \<open>variables \<Rightarrow> exp \<Rightarrow> val \<Rightarrow> bool\<close> (\<open>_ \<turnstile> _ \<leadsto>* _\<close>)
 where
@@ -609,5 +518,10 @@ lemma REDUCE:
       and \<open>\<Delta> \<turnstile> e\<^sub>2 \<leadsto>* v\<close>
     shows \<open>\<Delta> \<turnstile> e\<^sub>1 \<leadsto>* v\<close>
   using assms sorry
+
+
+
+(* THERE is a lot that needs to be done *)
+
 
 end
