Typing.thy
@@ -53,18 +53,18 @@ fun
 where
   \<open>typing_expression_val \<Gamma> (Immediate (num \<Colon> sz')) (Imm sz) = (sz = sz' \<and> sz > 0 \<and> (\<Gamma> is ok))\<close> |
   \<open>typing_expression_val \<Gamma> (Unknown str t) t' = (t = t' \<and> (t is ok) \<and> (\<Gamma> is ok))\<close> |
-  \<open>typing_expression_val \<Gamma> (Storage v w v' sz) (Mem sz\<^sub>a\<^sub>d\<^sub>d\<^sub>r sz') = (sz = sz' \<and> sz > 0 \<and> sz\<^sub>a\<^sub>d\<^sub>d\<^sub>r > 0 \<and> 
-       (\<Gamma> \<turnstile> v' :: (Imm sz)) \<and> bits w = sz\<^sub>a\<^sub>d\<^sub>d\<^sub>r \<and> (\<Gamma> \<turnstile> v :: (Mem sz\<^sub>a\<^sub>d\<^sub>d\<^sub>r sz')))\<close> |
+  \<open>typing_expression_val \<Gamma> (Storage v (num \<Colon> sz\<^sub>a\<^sub>d\<^sub>d\<^sub>r') v' sz) (Mem sz\<^sub>a\<^sub>d\<^sub>d\<^sub>r sz') = (sz = sz' \<and> sz > 0 \<and> sz\<^sub>a\<^sub>d\<^sub>d\<^sub>r > 0 \<and> 
+       (\<Gamma> \<turnstile> v' :: (Imm sz)) \<and> sz\<^sub>a\<^sub>d\<^sub>d\<^sub>r' = sz\<^sub>a\<^sub>d\<^sub>d\<^sub>r \<and> (\<Gamma> \<turnstile> v :: (Mem sz\<^sub>a\<^sub>d\<^sub>d\<^sub>r sz')))\<close> |
   \<open>typing_expression_val \<Gamma> v t = False\<close>
 fun 
   typing_expression_exp :: \<open>TypingContext \<Rightarrow> exp \<Rightarrow> Type \<Rightarrow> bool\<close>
 where
   \<open>typing_expression_exp \<Gamma> (Var (name, t')) t = (t = t' \<and> (name, t') \<in> set \<Gamma> \<and> (\<Gamma> is ok))\<close> |
-  \<open>typing_expression_exp \<Gamma> (Load e\<^sub>1 e\<^sub>2 ed sz') (Imm sz'') = (sz'' = sz' \<and> sz' > 0 \<and> (\<exists>sz sz\<^sub>m\<^sub>e\<^sub>m. sz' mod sz = 0 \<and> 
-                                             (\<Gamma> \<turnstile> e\<^sub>1 :: (Mem sz\<^sub>m\<^sub>e\<^sub>m sz)) \<and> (\<Gamma> \<turnstile> e\<^sub>2 :: (Imm sz\<^sub>m\<^sub>e\<^sub>m))))\<close> |
-  \<open>typing_expression_exp \<Gamma> (Store e\<^sub>1 e\<^sub>2 ed sz' e\<^sub>3) (Mem sz\<^sub>m\<^sub>e\<^sub>m sz) = (sz' mod sz = 0 \<and> sz' > 0 \<and> (\<Gamma> \<turnstile> e\<^sub>3 :: (Imm sz'))
-                                                    \<and> (\<Gamma> \<turnstile> e\<^sub>2 :: (Imm sz\<^sub>m\<^sub>e\<^sub>m)) 
-                                                    \<and> (\<Gamma> \<turnstile> e\<^sub>1 :: (Mem sz\<^sub>m\<^sub>e\<^sub>m sz)))\<close> |
+  \<open>typing_expression_exp \<Gamma> (Load e\<^sub>1 e\<^sub>2 ed sz) (Imm sz') = (sz' = sz \<and> sz > 0 \<and> (\<exists>sz\<^sub>m\<^sub>e\<^sub>m sz\<^sub>a\<^sub>d\<^sub>d\<^sub>r. sz mod sz\<^sub>m\<^sub>e\<^sub>m = 0 \<and> 
+                                             (\<Gamma> \<turnstile> e\<^sub>1 :: (Mem sz\<^sub>a\<^sub>d\<^sub>d\<^sub>r sz\<^sub>m\<^sub>e\<^sub>m)) \<and> (\<Gamma> \<turnstile> e\<^sub>2 :: (Imm sz\<^sub>a\<^sub>d\<^sub>d\<^sub>r))))\<close> |
+  \<open>typing_expression_exp \<Gamma> (Store e\<^sub>1 e\<^sub>2 ed sz e\<^sub>3) (Mem sz\<^sub>a\<^sub>d\<^sub>d\<^sub>r sz\<^sub>m\<^sub>e\<^sub>m) = (sz mod sz\<^sub>m\<^sub>e\<^sub>m = 0 \<and> sz > 0 \<and> (\<Gamma> \<turnstile> e\<^sub>3 :: (Imm sz))
+                                                    \<and> (\<Gamma> \<turnstile> e\<^sub>2 :: (Imm sz\<^sub>a\<^sub>d\<^sub>d\<^sub>r)) 
+                                                    \<and> (\<Gamma> \<turnstile> e\<^sub>1 :: (Mem sz\<^sub>a\<^sub>d\<^sub>d\<^sub>r sz\<^sub>m\<^sub>e\<^sub>m)))\<close> |
   \<open>typing_expression_exp \<Gamma> (BinOp e\<^sub>1 (AOp aop) e\<^sub>2) (Imm sz) = ((\<Gamma> \<turnstile> e\<^sub>1 :: (Imm sz)) \<and> (\<Gamma> \<turnstile> e\<^sub>2 :: (Imm sz)))\<close> |
   \<open>typing_expression_exp \<Gamma> (BinOp e\<^sub>1 (LOp lop) e\<^sub>2) (Imm (Suc 0)) = (\<exists>sz. (\<Gamma> \<turnstile> e\<^sub>1 :: (Imm sz)) \<and> (\<Gamma> \<turnstile> e\<^sub>2 :: (Imm sz)))\<close> | 
   \<open>typing_expression_exp \<Gamma> (UnOp uop e) (Imm sz) = (\<Gamma> \<turnstile> e :: (Imm sz))\<close> |
@@ -81,6 +81,112 @@ where
   \<open>typing_expression_exp \<Gamma> e t = False\<close>
 end
 
+lemma typing_val_storage:
+  assumes \<open>\<Gamma> \<turnstile> (Storage v w v' sz\<^sub>m\<^sub>e\<^sub>m) :: (Mem sz\<^sub>a\<^sub>d\<^sub>d\<^sub>r sz\<^sub>m\<^sub>e\<^sub>m')\<close>
+    shows \<open>bits w = sz\<^sub>a\<^sub>d\<^sub>d\<^sub>r \<and> sz\<^sub>m\<^sub>e\<^sub>m = sz\<^sub>m\<^sub>e\<^sub>m' \<and> sz\<^sub>m\<^sub>e\<^sub>m > 0 \<and> sz\<^sub>a\<^sub>d\<^sub>d\<^sub>r > 0 \<and> 
+       (\<Gamma> \<turnstile> v' :: (Imm sz\<^sub>m\<^sub>e\<^sub>m)) \<and> (\<Gamma> \<turnstile> v :: (Mem sz\<^sub>a\<^sub>d\<^sub>d\<^sub>r sz\<^sub>m\<^sub>e\<^sub>m))\<close>
+  using assms by (metis Bitvector_Syntax.word.exhaust typing_expression_val.simps(3) word.sel(2))
+
+lemma typing_val_immediate:
+  assumes \<open>\<Gamma> \<turnstile> (Immediate w) :: (Imm sz)\<close>
+    shows \<open>sz = bits w \<and> sz > 0 \<and> (\<Gamma> is ok)\<close>
+  using assms by (metis Bitvector_Syntax.word.exhaust typing_expression_val.simps(1) word.sel(2))
+
+text \<open>Better induction rule for val\<close>
+
+
+
+lemma typing_val_implies_valid_t:
+  assumes \<open>\<Gamma> \<turnstile> (v::val) :: t\<close>
+    shows \<open>t is ok\<close>
+  using assms by (induct rule: typing_expression_val.induct, auto)
+
+lemma typing_val_implies_valid_context:
+  assumes \<open>\<Gamma> \<turnstile> (v::val) :: t\<close>
+    shows \<open>\<Gamma> is ok\<close>
+  using assms by (induct rule: typing_expression_val.induct, auto)
+
+lemma typing_expression_val_induct[consumes 1, case_names Immediate Storage Unknown]:
+  assumes \<open>\<Gamma> \<turnstile> v :: t\<close>
+      and \<open>(\<And> num sz t. \<lbrakk>\<Gamma> is ok; sz > 0; t = Imm sz\<rbrakk> 
+                \<Longrightarrow> P (Immediate (num \<Colon> sz)) (Imm sz))\<close>
+      and \<open>(\<And>num sz\<^sub>a\<^sub>d\<^sub>d\<^sub>r sz\<^sub>v\<^sub>a\<^sub>l v v' t. \<lbrakk>\<Gamma> is ok; sz\<^sub>v\<^sub>a\<^sub>l > 0; sz\<^sub>a\<^sub>d\<^sub>d\<^sub>r > 0; t = Mem sz\<^sub>a\<^sub>d\<^sub>d\<^sub>r sz\<^sub>v\<^sub>a\<^sub>l;
+              \<Gamma> \<turnstile> v :: (Mem sz\<^sub>a\<^sub>d\<^sub>d\<^sub>r sz\<^sub>v\<^sub>a\<^sub>l); P v (Mem sz\<^sub>a\<^sub>d\<^sub>d\<^sub>r sz\<^sub>v\<^sub>a\<^sub>l);
+              \<Gamma> \<turnstile> v' :: (Imm sz\<^sub>v\<^sub>a\<^sub>l); P v' (Imm sz\<^sub>v\<^sub>a\<^sub>l)\<rbrakk> 
+                \<Longrightarrow> P (Storage v (num \<Colon> sz\<^sub>a\<^sub>d\<^sub>d\<^sub>r) v' sz\<^sub>v\<^sub>a\<^sub>l) (Mem sz\<^sub>a\<^sub>d\<^sub>d\<^sub>r sz\<^sub>v\<^sub>a\<^sub>l))\<close>
+      and \<open>(\<And>str t. \<lbrakk>\<Gamma> is ok; t is ok\<rbrakk> 
+                \<Longrightarrow> P (Unknown str t) t)\<close>
+    shows \<open>P v t\<close>
+  using assms typing_val_implies_valid_context apply (induct rule: typing_expression_val.induct)
+  by auto
+
+lemma typing_expression_\<Gamma>_extend_implies_\<Gamma>:
+  fixes v :: val
+  assumes \<open>(name, t') # \<Gamma> \<turnstile> v :: t\<close> 
+    shows \<open>\<Gamma> \<turnstile> v :: t\<close>
+  using assms by (induct rule: typing_expression_val_induct, auto)
+
+lemma typing_expression_exp_induct_Let_intermediate:
+  assumes \<open>\<Gamma> \<turnstile> e :: t\<close>
+      and \<open>e = (Let (name, t') e\<^sub>1 e\<^sub>2)\<close>
+      and \<open>(\<lbrakk>\<Gamma> \<turnstile> e\<^sub>1 :: t'; ((name, t') # \<Gamma>) \<turnstile> e\<^sub>2 :: t\<rbrakk> \<Longrightarrow> P (Let (name, t') e\<^sub>1 e\<^sub>2) t)\<close> 
+    shows \<open>P e t\<close>
+  using assms by auto
+
+
+lemma typing_expression_exp_induct[consumes 1, case_names Val Var Load Store BinAOp BinLOp UOp
+                                               UnsignedCast SignedCast HighCast LowCast Let Ite 
+                                               Extract Concat]:
+  assumes \<open>\<Gamma> \<turnstile> e :: t\<close>
+      and \<open>(\<And>\<Gamma> v t. \<Gamma> \<turnstile> v :: t 
+              \<Longrightarrow> P \<Gamma> (Val v) t)\<close>
+      and \<open>(\<And>\<Gamma> name t. \<lbrakk>(name, t) \<in> set \<Gamma>; (\<Gamma> is ok)\<rbrakk> 
+              \<Longrightarrow> P \<Gamma> (Var (name, t)) t)\<close>
+      and \<open>(\<And>\<Gamma> e\<^sub>1 e\<^sub>2 ed sz sz\<^sub>a\<^sub>d\<^sub>d\<^sub>r sz\<^sub>m\<^sub>e\<^sub>m t. \<lbrakk>sz > 0; sz mod sz\<^sub>m\<^sub>e\<^sub>m = 0; t = Imm sz; 
+                \<Gamma> \<turnstile> e\<^sub>1 :: (Mem sz\<^sub>a\<^sub>d\<^sub>d\<^sub>r sz\<^sub>m\<^sub>e\<^sub>m); P \<Gamma> e\<^sub>1 (Mem sz\<^sub>a\<^sub>d\<^sub>d\<^sub>r sz\<^sub>m\<^sub>e\<^sub>m); 
+                \<Gamma> \<turnstile> e\<^sub>2 :: (Imm sz\<^sub>a\<^sub>d\<^sub>d\<^sub>r); P \<Gamma> e\<^sub>2 (Imm sz\<^sub>a\<^sub>d\<^sub>d\<^sub>r)\<rbrakk> 
+              \<Longrightarrow> P \<Gamma> (Load e\<^sub>1 e\<^sub>2 ed sz) (Imm sz))\<close>
+      and \<open>(\<And>\<Gamma> sz\<^sub>a\<^sub>d\<^sub>d\<^sub>r sz\<^sub>m\<^sub>e\<^sub>m sz\<^sub>v\<^sub>a\<^sub>l e\<^sub>1 e\<^sub>2 ed e\<^sub>3 t. \<lbrakk>sz\<^sub>v\<^sub>a\<^sub>l mod sz\<^sub>m\<^sub>e\<^sub>m = 0; sz\<^sub>v\<^sub>a\<^sub>l > 0; t = Mem sz\<^sub>a\<^sub>d\<^sub>d\<^sub>r sz\<^sub>m\<^sub>e\<^sub>m;
+                \<Gamma> \<turnstile> e\<^sub>3 :: (Imm sz\<^sub>v\<^sub>a\<^sub>l); P \<Gamma> e\<^sub>3 (Imm sz\<^sub>v\<^sub>a\<^sub>l);
+                \<Gamma> \<turnstile> e\<^sub>2 :: (Imm sz\<^sub>a\<^sub>d\<^sub>d\<^sub>r); P \<Gamma> e\<^sub>2 (Imm sz\<^sub>a\<^sub>d\<^sub>d\<^sub>r);
+                \<Gamma> \<turnstile> e\<^sub>1 :: (Mem sz\<^sub>a\<^sub>d\<^sub>d\<^sub>r sz\<^sub>m\<^sub>e\<^sub>m); P \<Gamma> e\<^sub>1 (Mem sz\<^sub>a\<^sub>d\<^sub>d\<^sub>r sz\<^sub>m\<^sub>e\<^sub>m)\<rbrakk> 
+              \<Longrightarrow> P \<Gamma> (Store e\<^sub>1 e\<^sub>2 ed sz\<^sub>v\<^sub>a\<^sub>l e\<^sub>3) (Mem sz\<^sub>a\<^sub>d\<^sub>d\<^sub>r sz\<^sub>m\<^sub>e\<^sub>m))\<close>
+      and \<open>(\<And>\<Gamma> e\<^sub>1 aop e\<^sub>2 sz t. \<lbrakk>t = Imm sz; 
+                \<Gamma> \<turnstile> e\<^sub>1 :: (Imm sz); P \<Gamma> e\<^sub>1 (Imm sz); 
+                \<Gamma> \<turnstile> e\<^sub>2 :: (Imm sz); P \<Gamma> e\<^sub>2 (Imm sz)\<rbrakk> 
+              \<Longrightarrow> P \<Gamma> (BinOp e\<^sub>1 (AOp aop) e\<^sub>2) (Imm sz))\<close>
+      and \<open>(\<And>\<Gamma> e\<^sub>1 lop e\<^sub>2 sz t. \<lbrakk>t = Imm 1;
+                \<Gamma> \<turnstile> e\<^sub>1 :: (Imm sz); P \<Gamma> e\<^sub>1 (Imm sz);
+                \<Gamma> \<turnstile> e\<^sub>2 :: (Imm sz); P \<Gamma> e\<^sub>2 (Imm sz)\<rbrakk> 
+              \<Longrightarrow> P \<Gamma> (BinOp e\<^sub>1 (LOp lop) e\<^sub>2) (Imm 1))\<close>
+      and \<open>(\<And>\<Gamma> uop e sz t. \<lbrakk>t = Imm sz; \<Gamma> \<turnstile> e :: (Imm sz); P \<Gamma> e (Imm sz)\<rbrakk> 
+              \<Longrightarrow> P \<Gamma> (UnOp uop e) (Imm sz))\<close>
+      and \<open>(\<And>\<Gamma> e sz sz' t. \<lbrakk>sz \<ge> sz'; \<Gamma> \<turnstile> e :: (Imm sz'); sz > 0; t = Imm sz; P \<Gamma> e (Imm sz')\<rbrakk> 
+              \<Longrightarrow> P \<Gamma> (Cast Unsigned sz e) (Imm sz))\<close>
+      and \<open>(\<And>\<Gamma> e sz sz' t. \<lbrakk>sz \<ge> sz'; \<Gamma> \<turnstile> e :: (Imm sz'); sz > 0; t = Imm sz; P \<Gamma> e (Imm sz')\<rbrakk>
+              \<Longrightarrow> P \<Gamma> (Cast Signed sz e) (Imm sz))\<close>
+      and \<open>(\<And>\<Gamma> e sz sz' t. \<lbrakk>sz' \<ge> sz; \<Gamma> \<turnstile> e :: (Imm sz'); sz > 0; t = Imm sz; P \<Gamma> e (Imm sz')\<rbrakk>
+              \<Longrightarrow> P \<Gamma> (Cast High sz e) (Imm sz))\<close>
+      and \<open>(\<And>\<Gamma> e sz sz' t. \<lbrakk>sz' \<ge> sz; \<Gamma> \<turnstile> e :: (Imm sz'); sz > 0; t = Imm sz; P \<Gamma> e (Imm sz')\<rbrakk>
+              \<Longrightarrow> P \<Gamma> (Cast Low sz e) (Imm sz))\<close>
+      and \<open>(\<And>\<Gamma> name t' e\<^sub>1 e\<^sub>2 t. \<lbrakk>\<Gamma> \<turnstile> e\<^sub>1 :: t'; P \<Gamma> e\<^sub>1 t';
+                ((name, t') # \<Gamma>) \<turnstile> e\<^sub>2 :: t; P ((name, t') # \<Gamma>) e\<^sub>2 t\<rbrakk> 
+              \<Longrightarrow> P \<Gamma> (Let (name, t') e\<^sub>1 e\<^sub>2) t)\<close>
+      and \<open>(\<And>\<Gamma> e\<^sub>1 e\<^sub>2 e\<^sub>3 t. \<lbrakk>\<Gamma> \<turnstile> e\<^sub>1 :: (Imm 1); P \<Gamma> e\<^sub>1 (Imm 1);
+                \<Gamma> \<turnstile> e\<^sub>2 :: t; P \<Gamma> e\<^sub>2 t;
+                \<Gamma> \<turnstile> e\<^sub>3 :: t; P \<Gamma> e\<^sub>3 t\<rbrakk> 
+              \<Longrightarrow> P \<Gamma> (Ite e\<^sub>1 e\<^sub>2 e\<^sub>3) t)\<close>
+      and \<open>(\<And>\<Gamma> sz\<^sub>1 sz\<^sub>2 sz\<^sub>e\<^sub>x\<^sub>t\<^sub>r\<^sub>a\<^sub>c\<^sub>t sz e t. \<lbrakk>sz\<^sub>e\<^sub>x\<^sub>t\<^sub>r\<^sub>a\<^sub>c\<^sub>t = sz\<^sub>1 - sz\<^sub>2 + 1; sz\<^sub>1 \<ge> sz\<^sub>2; t = Imm sz\<^sub>e\<^sub>x\<^sub>t\<^sub>r\<^sub>a\<^sub>c\<^sub>t; 
+                \<Gamma> \<turnstile> e :: (Imm sz); P \<Gamma> e (Imm sz)\<rbrakk> 
+              \<Longrightarrow> P \<Gamma> (Extract sz\<^sub>1 sz\<^sub>2 e) (Imm sz\<^sub>e\<^sub>x\<^sub>t\<^sub>r\<^sub>a\<^sub>c\<^sub>t))\<close>
+      and \<open>(\<And>\<Gamma> e\<^sub>1 e\<^sub>2 sz\<^sub>c\<^sub>o\<^sub>n\<^sub>c\<^sub>a\<^sub>t sz\<^sub>1 sz\<^sub>2 t. \<lbrakk>sz\<^sub>c\<^sub>o\<^sub>n\<^sub>c\<^sub>a\<^sub>t = sz\<^sub>1 + sz\<^sub>2; t = Imm sz\<^sub>c\<^sub>o\<^sub>n\<^sub>c\<^sub>a\<^sub>t;
+                \<Gamma> \<turnstile> e\<^sub>1 :: (Imm sz\<^sub>1); P \<Gamma> e\<^sub>1 (Imm sz\<^sub>1); 
+                \<Gamma> \<turnstile> e\<^sub>2 :: (Imm sz\<^sub>2); P \<Gamma> e\<^sub>2 (Imm sz\<^sub>2)\<rbrakk> 
+              \<Longrightarrow> P \<Gamma> (Concat e\<^sub>1 e\<^sub>2) (Imm sz\<^sub>c\<^sub>o\<^sub>n\<^sub>c\<^sub>a\<^sub>t))\<close>
+    shows \<open>P \<Gamma> e t\<close>
+  using assms apply (induct rule: typing_expression_exp.induct)
+  apply auto
+  by presburger
 
 consts judgement_is_ok :: \<open>TypingContext \<Rightarrow> 'a \<Rightarrow> bool\<close> (\<open>_ \<turnstile> _ is ok\<close>)
 
